theories/Common.v
@@ -1,0 +1,6 @@
+Require Export MPST.Common.Forall.
+Require Export MPST.Common.Member.
+Require Export MPST.Common.AtomSets.
+Require Export MPST.Common.Actions.
+Require Export MPST.Common.Queue.
+Require Export MPST.Common.Alt.
