theories/Common/Actions.v
@@ -1,0 +1,53 @@
+From mathcomp.ssreflect Require Import all_ssreflect.
+Set Implicit Arguments.
+Unset Strict Implicit.
+Import Prenex Implicits.
+
+Require Import MPST.Common.AtomSets.
+
+Inductive l_act := l_send | l_recv.
+
+Definition dual_act a :=
+  match a with
+  | l_send => l_recv
+  | l_recv => l_send
+  end.
+
+Create HintDb mpst.
+
+Lemma dual_actK a : dual_act (dual_act a) = a.
+Proof. by case: a. Qed.
+Hint Rewrite dual_actK : mpst.
+
+Definition eq_lact a b :=
+  match a, b with
+  | l_send, l_send
+  | l_recv, l_recv => true
+  | _, _ => false
+  end.
+
+Lemma lact_eqP : Equality.axiom eq_lact.
+Proof. by rewrite /Equality.axiom => [[] []/=]; constructor. Qed.
+
+Definition lact_eqMixin := EqMixin lact_eqP.
+Canonical lact_eqType := Eval hnf in EqType l_act lact_eqMixin.
+
+
+Inductive act :=
+| mk_act (a : l_act) (p : role) (q : role) (l : lbl) (t : mty).
+
+(* a trace is simply a stream of actions *)
+CoInductive trace (act : Type) :=
+| tr_end : trace act
+| tr_next : act -> trace act -> trace act.
+
+CoFixpoint trace_map {A B : Type} (f : A -> B) (trc : trace A) : trace B :=
+  match trc with
+  | tr_end => tr_end _
+  | tr_next a trc => tr_next (f a) (trace_map f trc)
+  end
+.
+
+Definition subject A := let: mk_act a p q _ _ := A in p.
+Definition object A := let: mk_act a p q _ _ := A in q.
+Definition act_ty A := let: mk_act a _ _ _ _ := A in a.
