theories/Common/Queue.v
@@ -1,0 +1,29 @@
+From mathcomp.ssreflect Require Import all_ssreflect.
+Set Implicit Arguments.
+Unset Strict Implicit.
+Import Prenex Implicits.
+
+Require Import MPST.Common.AtomSets.
+
+Definition MsgQ := seq ((role * role) * seq (lbl * mty)).
+
+Fixpoint enqueue (A : eqType) B (p : seq (A * seq B)) (x : A * B) :=
+  match p with
+  | [::] => [:: (x.1, [:: x.2])]
+  | h :: t => if h.1 == x.1 then (h.1, h.2 ++ [:: x.2]) :: t
+              else h :: enqueue t x
+  end.
+
+Fixpoint dequeue (A : eqType) B (p : seq (A * seq B)) (x : A)
+  : option (B * seq (A * seq B)) :=
+  match p with
+  | [::] => None
+  | h :: t => if h.1 == x then match h.2 with
+                               | [::] => None
+                               | f :: q => Some (f, (h.1, q) :: t)
+                               end
+              else match dequeue t x with
+                   | None => None
+                   | Some (e, t') => Some (e, h :: t')
+                   end
+  end.
