theories/Global/Syntax.v
@@ -1,0 +1,453 @@
+From mathcomp.ssreflect Require Import all_ssreflect seq.
+From mathcomp Require Import finmap.
+
+From Paco Require Import paco paco2.
+
+Set Implicit Arguments.
+Unset Strict Implicit.
+Import Prenex Implicits.
+
+Require Import MPST.Common.
+
+Unset Elimination Schemes.
+(**
+ * Global Types
+ *)
+Inductive g_ty :=
+| g_end
+| g_var (VAR : nat)
+| g_rec (GT : g_ty)
+| g_msg (FROM TO : role) (CONT : seq (lbl * (mty * g_ty))).
+Hint Constructors g_ty : mpst.
+Set Elimination Schemes.
+
+Lemma g_ty_ind :
+  forall (P : g_ty -> Prop),
+    P g_end ->
+    (forall v, P (g_var v)) ->
+    (forall G, P G -> P (g_rec G)) ->
+    (forall p q Ks, (forall K, member K Ks -> P K.2.2) ->
+                      P (g_msg p q Ks)) ->
+    forall g : g_ty, P g.
+Proof.
+  move=> P P_end P_var P_rec P_msg; fix Ih 1; case.
+  + by apply: P_end.
+  + by apply: P_var.
+  + by move=>G; apply: P_rec.
+  + move=>p q Ks; apply: P_msg.
+    by apply/forall_member; elim: Ks.
+Qed.
+
+Fixpoint depth (a : g_ty) :=
+  match a with
+  | g_end
+  | g_var _ => 0
+  | g_rec G => (depth G).+1
+  | g_msg _ _ K => (foldr maxn 0 (map (fun x=> depth x.2.2) K)).+1
+  end.
+
+Fixpoint participants (G : g_ty) :=
+  match G with
+  | g_end
+  | g_var _ => [::]
+  | g_rec G => participants G
+  | g_msg p q Ks => p::q::flatten [seq participants K.2.2 | K <- Ks]
+  end.
+
+Fixpoint eq_g_ty (a b : g_ty) :=
+  match a, b with
+  | g_end, g_end => true
+  | g_var v1, g_var v2 => v1 == v2
+  | g_rec G1, g_rec G2 => eq_g_ty G1 G2
+  | g_msg p1 q1 Ks1, g_msg p2 q2 Ks2 =>
+      (p1 == p2)
+      && (q1 == q2)
+      && (fix eqL Ks1 Ks2 :=
+            match Ks1, Ks2 with
+            | [::], [::] => true
+            | K1::Ks1, K2::Ks2 => (K1.1 == K2.1)
+                                    && (K1.2.1 == K2.2.1)
+                                    && eq_g_ty K1.2.2 K2.2.2
+                                    && eqL Ks1 Ks2
+            | _, _ => false
+            end) Ks1 Ks2
+  | _, _ => false
+  end.
+
+Definition eq_alt (l r : lbl * (mty * g_ty)) :=
+  (l.1 == r.1) && (l.2.1 == r.2.1) && eq_g_ty l.2.2 r.2.2.
+
+Lemma eqgty_all p1 q1 (Ks1 : seq (lbl * (mty * g_ty))) p2 q2 Ks2 :
+  eq_g_ty (g_msg p1 q1 Ks1) (g_msg p2 q2 Ks2) =
+  (p1 == p2) && (q1 == q2) && all2 eq_alt Ks1 Ks2.
+Proof.
+  rewrite /=; do 2 (case: eqP=>///= _).
+Qed.
+Hint Rewrite eqgty_all : mpst.
+
+Lemma g_ty_eqP : Equality.axiom eq_g_ty.
+Proof.
+  rewrite /Equality.axiom; fix Ih 1 => x y.
+  case x =>[|vl| Gl |pl ql Ksl]; case y =>[|vr| Gr |pr qr Ksr];
+    try (by constructor).
+  + by rewrite /eq_g_ty; case: eqP=>[->|H];constructor=>//[[]].
+  + by rewrite /=; case: Ih=>[->|H];constructor=>//[[]].
+  + rewrite eqgty_all; do 2 (case: eqP=>[<-|H];[|constructor=>[[]]//] =>/=).
+    elim: Ksl Ksr =>[|[ll [tl Gl]] Ksl IhKs].
+    - case; try (by constructor).
+    - move=>[|[lr [tr Gr] Ksr]/=]; first (by constructor).
+      rewrite /eq_alt/=; do 2 (case: eqP=>[->|F];[|constructor=>[[/F]]//]).
+      case: Ih=>[->|F]/=;[|constructor=>[[/F]]//].
+      by case: IhKs=>[[]<-|F]; constructor=>//[[F']]; move: F' F=>->.
+Qed.
+
+Definition g_ty_eqMixin := EqMixin g_ty_eqP.
+Canonical g_ty_eqType := Eval hnf in EqType g_ty g_ty_eqMixin.
+
+Lemma alt_eqP : Equality.axiom eq_alt.
+Proof.
+  rewrite /Equality.axiom/eq_alt; move=>[l1  [t1 Ks1]] [l2 [t2 Ks2]]/=.
+  do 2 (case: eqP=>[<-|H]; last (by apply: ReflectF => [[/H]])).
+  case: g_ty_eqP=>[<-|H]; first by apply: ReflectT.
+  by apply: ReflectF =>[[/H]].
+Qed.
+
+Lemma rec_gty G :
+  (exists G', G = g_rec G') \/ (forall G', G != g_rec G').
+Proof. by case:G; try (by right); move=> GT; left; exists GT. Qed.
+
+Lemma matchGrec A G (f : g_ty -> A) g :
+  (forall G', G != g_rec G') ->
+  match G with
+  | g_rec G' => f G'
+  | _ => g
+  end = g.
+Proof. by case: G=>// GT /(_ GT)/eqP. Qed.
+
+(**
+ * Does not apply any "shift" to G2, and therefore G2 must always be closed
+ *)
+Fixpoint g_open (d : nat) (G2 : g_ty) (G1 : g_ty) :=
+  match G1 with
+  | g_end => G1
+  | g_var v => if v == d then G2 else G1
+  | g_rec G => g_rec (g_open d.+1 G2 G)
+  | g_msg p q Ks =>
+    g_msg p q [seq (K.1, (K.2.1, g_open d G2 K.2.2)) | K <- Ks]
+  end.
+Notation "{ k '~>' v } G":= (g_open k v G) (at level 30, right associativity).
+Notation "G '^' v":= (g_open 0 (g_var v) G) (at level 30, right associativity).
+
+Definition unroll G := g_open 0 (g_rec G) G.
+
+Lemma g_open_msg_rw d G2 FROM TO CONT:
+  g_open d G2 (g_msg FROM TO CONT)
+  = g_msg FROM TO [seq (K.1, (K.2.1, g_open d G2 K.2.2)) | K <- CONT].
+Proof. by []. Qed.
+
+Lemma notin_part_g_open_strong d r G G': r \notin participants G ->
+  r \notin participants G'-> r \notin participants (g_open d G' G).
+Proof.
+move=> h1 rnG'; move: h1; apply: contra; elim: G d.
++ rewrite //=.
++ rewrite //= => v d.
+  by case: ifP=>[_ F|//]; rewrite F in rnG'.
++ rewrite //=. by move=> G ih d; apply ih.
++ move=>p q Ks ih d. rewrite /= !in_cons -map_comp/comp/=.
+  move=>/orP-[->//|/orP-[->|]]; first by rewrite orbC.
+  move=> H.
+  do ! (apply/orP; right).
+  move: H=>/flatten_mapP-[K inKs inK].
+  apply/flatten_mapP.
+  exists K=>//.
+  by apply: (ih _ _ d); first by apply/memberP.
+Qed.
+
+Lemma same_notin_part_g_open d r G G': participants G' = participants G ->
+  r \notin participants G -> r \notin participants (g_open d G' G).
+Proof.
+  move=>h1 h2; apply: notin_part_g_open_strong; by [apply h2 | rewrite h1].
+Qed.
+
+Lemma notin_part_g_open r G:
+  r \notin participants G -> r \notin participants (g_open 0 (g_rec G) G).
+Proof.
+  by apply same_notin_part_g_open; rewrite //=.
+Qed.
+
+Fixpoint g_fidx (d : nat) (G : g_ty) : seq nat :=
+  match G with
+  | g_var v => if v >= d then [:: v - d] else [::]
+  | g_rec G => g_fidx d.+1 G
+  | g_msg p q Ks => flatten [seq g_fidx d K.2.2 | K <- Ks]
+  | g_end => [::]
+  end.
+Definition g_closed (G : g_ty) := g_fidx 0 G == [::].
+
+Lemma gfbvar_next n G :
+  g_fidx n G == fset0 ->
+  g_fidx n.+1 G = fset0.
+Proof.
+  elim: G n=>[//|v|G Ih|p q Ks Ih] n/=.
+  - case: v=>//= m H; case: ifP=>// n_m; move: H.
+    by move: (leq_trans (leqnSn n) n_m)=>->.
+  - by apply: Ih.
+  - rewrite flatten_eq_nil member_map=>H; apply/eqP.
+    by rewrite flatten_eq_nil member_map=> K M; move: (Ih K M n (H K M))=>->.
+Qed.
+
+Fixpoint guarded d G :=
+  match G with
+  | g_end => true
+  | g_var v => v >= d
+  | g_rec G => guarded d.+1 G
+  | g_msg _ _ Ks => all (fun K => guarded 0 K.2.2) Ks
+  end.
+
+Fixpoint g_binds n G :=
+  match G with
+  | g_var v => v == n
+  | g_rec G => g_binds n.+1 G
+  | _ => false
+  end.
+
+Fixpoint guarded' G :=
+  match G with
+  | g_end
+  | g_var _ => true
+  | g_rec G => ~~ g_binds 0 G && guarded' G
+  | g_msg _ _ Ks => all (fun K => guarded' K.2.2) Ks
+  end.
+
+Lemma guarded_next n G : guarded n.+1 G = ~~ g_binds n G && guarded n G.
+Proof. by elim: G n=>//= v n; rewrite ltn_neqAle eq_sym. Qed.
+
+Lemma guarded_binds G : guarded 0 G = guarded' G.
+Proof.
+  elim: G=>[||G|_ _ Ks Ih]//=; first by move=><-;apply/guarded_next.
+  elim: Ks Ih=>[//|K Ks Ih']/= Ih; rewrite Ih; last by left.
+  by rewrite Ih' // => K' /or_intror/Ih.
+Qed.
+
+Lemma alt_eq p1 q1 Ks1 p2 q2 Ks2 :
+  ((g_msg p1 q1 Ks1) == (g_msg p2 q2 Ks2)) =
+  (p1 == p2) && (q1 == q2) && (Ks1 == Ks2).
+Proof.
+  rewrite eqE/=; do 2 case: eqP=>//=; move=> _ _ {p1 q1 p2 q2}.
+  elim: Ks1=>[|K1 Ks1 Ih] in Ks2 *; case: Ks2=>[|K2 Ks2]//=.
+  by rewrite Ih; do ! rewrite !eqE/=; rewrite -!eqE !andbA.
+Qed.
+
+Lemma gty_not_var A G (f : nat -> A) (k : A) :
+  (forall v : nat, G != g_var v) ->
+  match G with | g_var v => f v | _ => k end = k.
+Proof. by case: G =>// v /(_ v)/eqP. Qed.
+
+Fixpoint rec_depth G :=
+  match G with
+  | g_rec G => (rec_depth G).+1
+  | _ => 0
+  end.
+
+Lemma rd_zero G :
+  (forall G' : g_ty, G != g_rec G') ->
+  rec_depth G = 0.
+Proof. by case: G=>// GT /(_ GT)/eqP. Qed.
+
+
+Fixpoint n_unroll d G :=
+  match d with
+  | 0 => G
+  | d.+1 =>
+    match G with
+    | g_rec G' => n_unroll d (unroll G')
+    | _ => G
+    end
+  end.
+
+Lemma r_in_unroll r G n:
+  r \in participants (n_unroll n G) -> r \in participants G.
+Proof.
+  apply: contraLR.
+  elim: n => [rewrite //= | n ih] in G *; case G; rewrite //=.
+  move=> G0 notinpart; apply ih.
+  unfold unroll; apply notin_part_g_open; by [].
+Qed.
+
+Lemma r_in_unroll_rec_depth r G:
+  r \in participants (n_unroll (rec_depth G) G) -> r \in participants G.
+Proof. by apply r_in_unroll. Qed.
+
+Lemma notin_nunroll r n G :
+  r \notin participants G ->
+  r \notin participants (n_unroll n G).
+Proof.
+  elim: n G=>//= n Ih G H.
+  by case: G H=>//= GT; rewrite /unroll=>/notin_part_g_open/Ih.
+Qed.
+
+Lemma guarded_match d G :
+  match G with
+  | g_var v => d < v
+  | _ => guarded d.+1 G
+  end ->
+  (exists v, (G == g_var v) && (d < v)) \/
+  (forall v, (G != g_var v)) /\ guarded d.+1 G.
+Proof.
+  case: G=>[|[]||]//=; try by right.
+  by move=> n d_n; left; exists n.+1; rewrite eq_refl.
+Qed.
+
+Lemma guarded_recdepth d G m :
+  guarded d G ->
+  m < d ->
+  forall G', rec_depth G = rec_depth ({m ~> G'} G).
+Proof.
+  elim: G=>[|n|G Ih|p q Ks Ih]//= in d m *.
+  - move=>dn md G; case: ifP=>[/eqP-E|ne//].
+    by move: E dn md=>-> /leq_ltn_trans-H /H; rewrite ltnn.
+  - by move=> GG md G'; rewrite (Ih _ m.+1 GG _ G').
+Qed.
+
+Lemma guarded_depth_gt n dG dG' G :
+  n <= dG' ->
+  guarded dG' G -> g_fidx n G == [::] -> guarded dG G.
+Proof.
+  elim: G =>[|m|G Ih|p q Ks Ih]// in n dG dG' *.
+  - by move=> /leq_trans-H /= /H->.
+  - by move=>/= LE; apply/Ih.
+Qed.
+
+Lemma gopen_closed G :
+   g_closed (g_rec G) ->
+   g_closed (g_open 0 (g_rec G) G).
+ Proof.
+   rewrite/g_closed/==>G_fbv; have: g_fidx 0 (g_rec G) == fset0 by [].
+   move: (g_rec G) => G' G'0.
+   elim: G 0 G'0 G_fbv=>[//|v|G Ih|p q Ks Ih] n G'0/=.
+   - move=> H; case: ifP=>[//|/=]; case: ifP=>//; move: H.
+     case: ifP=>//; rewrite ltn_neqAle =>/(rwP negPf).
+     rewrite negb_and negbK eq_sym; by move=>/orP-[->//|/negPf->].
+   - by apply: (Ih n.+1); rewrite gfbvar_next.
+   - rewrite -map_comp/comp/=; move=>/flatten_eq_nil/member_map-H.
+     by apply/flatten_eq_nil/member_map=>K M; apply: Ih=>//; apply: H.
+ Qed.
+
+Lemma closed_not_var G :
+  g_closed G ->
+  forall v, G != g_var v.
+Proof.
+  by rewrite /g_closed; case: G=>//= n; rewrite -cardfs_eq0 cardfs1.
+Qed.
+
+Lemma open_not_var d G G' :
+  g_closed G ->
+  (forall v, G' != g_var v) ->
+  forall v, {d ~> G} G' != g_var v.
+Proof. by case: G'=>// n _ /(_ n)/eqP. Qed.
+
+Lemma guarded_open d1 d2 G G' :
+  guarded 0 G' ->
+  g_closed G' ->
+  guarded d1 G ->
+  guarded d1 ({d2 ~> G'} G).
+Proof.
+  elim: G=>[|n|G Ih|p q Ks Ih]//= in d1 d2 *.
+  - by case: ifP=>// _ /(guarded_depth_gt d1 (leq0n 0))-H /H-{H}H.
+  - by apply/Ih.
+  - move=> GG' CG'; elim: Ks=>[|K Ks IhK]//= in Ih *.
+    move=>/andP-[GK GKs].
+    move: (Ih K (or_introl (erefl _)) 0 d2 GG' CG' GK)=>->//=.
+    apply/IhK=>// K0 MK0; by apply/(Ih K0 (or_intror MK0)).
+Qed.
+
+Lemma guarded_gt d d' G :
+  d >= d' ->
+  guarded d G ->
+  guarded d' G.
+Proof.
+  elim: G=>[|n|G Ih|p q Ks Ih]//= in d d' *.
+  - by move=>/leq_trans-H /H.
+  - by move=> H; apply/Ih.
+Qed.
+
+Lemma unroll_guarded G :
+  g_closed G ->
+  guarded 0 G ->
+  forall G', n_unroll (rec_depth G) G != g_rec G'.
+Proof.
+  move: {-2}(rec_depth G) (eq_refl (rec_depth G)) => n.
+  elim: n => [|n Ih]/= in G *; case: G=>// G n_rd CG GG; move: n_rd.
+  rewrite eqE/=-eqE => n_rd.
+  have/=GG': (guarded 0 (g_rec G)) by [].
+  move: n_rd; rewrite (guarded_recdepth GG' (ltn0Sn 0) (g_rec G))=>n_rd.
+  apply/Ih=>//; first by apply/gopen_closed.
+  by apply/guarded_open=>//; apply/guarded_gt; last by apply/GG'.
+Qed.
+
+Fixpoint is_end g :=
+  match g with
+  | g_rec g => is_end g
+  | g_end => true
+  | _ => false
+  end.
+
+Lemma recdepth_unroll g :
+  is_end g -> rec_depth g = rec_depth (unroll g).
+Proof.
+  move=>END; have: (is_end (g_rec g)) by [].
+  rewrite /unroll; move: (g_rec g)=>g' END'.
+  by elim: g 0 END=>// g Ih n /=/(Ih n.+1)->.
+Qed.
+
+Lemma isend_unroll g :
+  is_end g -> is_end (unroll g).
+Proof.
+  move=>END; have: (is_end (g_rec g)) by [].
+  rewrite /unroll; move: (g_rec g)=>g' END'.
+  by elim: g 0 END=>// g Ih n /=/(Ih n.+1)->.
+Qed.
+
+Fixpoint non_empty_cont G :=
+  match G with
+  | g_msg _ _ Ks => ~~ nilp Ks && all id [seq non_empty_cont K.2.2 | K <- Ks]
+  | g_rec G => non_empty_cont G
+  | _ => true
+  end.
+
+Definition g_precond G :=
+  g_closed G && guarded 0 G && non_empty_cont G.
+
+Lemma ne_open n G G' :
+  non_empty_cont G -> non_empty_cont G' -> non_empty_cont (g_open n G' G).
+Proof.
+  move=> NE1 NE2; move: NE1.
+  elim: G n=>//.
+  - by move=>v n; rewrite /unroll/=; case: ifP=>//.
+  - by move=> G Ih n /=; apply/Ih.
+  - move=> F T C Ih n /=; case: C Ih=>//= K Ks Ih /andP-[NE_K ALL].
+    rewrite (Ih K (or_introl erefl) n NE_K) /= {NE_K}.
+    move: Ih=>/(_ _ (or_intror _) n)=> Ih.
+    move: ALL=>/forallbP/forall_member/member_map-ALL.
+    apply/forallbP/forall_member/member_map/member_map=>/={}K M.
+    by apply/(Ih _ M)/ALL.
+Qed.
+
+Lemma ne_unr n G : non_empty_cont G -> non_empty_cont (n_unroll n G).
+Proof.
+  elim: n G=>[//|n/=] Ih; case=>//= G NE.
+  have: non_empty_cont (g_rec G) by [].
+  by move=>/(ne_open 0 NE); apply/Ih.
+Qed.
+
+
+Lemma precond_parts g :
+  g_precond g -> ~~ nilp (participants g) \/ is_end g.
+Proof.
+  move=>/andP-[/andP-[CG GG]  _]; move: CG GG; rewrite /g_closed.
+  elim: g 0.
+  - by move=> n _ _; right.
+  - by move=>v n /= H E; move: E H=>->.
+  - by move=> G Ih n /=; apply/Ih.
+  - by move=> p q Ks _ n  _ _; left.
+Qed.
