theories/Global/Tree.v
@@ -1,0 +1,167 @@
+From mathcomp.ssreflect Require Import all_ssreflect seq.
+From mathcomp Require Import finmap.
+
+From Paco Require Import paco paco2.
+
+Set Implicit Arguments.
+Unset Strict Implicit.
+Import Prenex Implicits.
+
+Require Import MPST.Common.
+
+CoInductive rg_ty :=
+| rg_end
+| rg_msg (FROM TO : role)
+         (CONT : lbl -> option (mty * rg_ty)).
+
+Unset Elimination Schemes.
+Inductive ig_ty :=
+| ig_end (CONT : rg_ty)
+| ig_msg (ST : option lbl)
+         (FROM TO : role)
+         (CONT : lbl -> option (mty * ig_ty)).
+Set Elimination Schemes.
+
+Definition P_option A (P : A -> Type) (C : option A) : Type :=
+  match C with
+  | Some X => P X
+  | None => True
+  end.
+
+Definition P_prod A B (P : B -> Type) (C : A * B) : Type :=
+  match C with
+  | (X, Y)=> P Y
+  end.
+
+Lemma ig_ty_ind'
+      (P : ig_ty -> Prop)
+      (P_end : forall CONT, P (ig_end CONT))
+      (P_msg : (forall ST FROM TO CONT,
+                   (forall L, P_option (P_prod P) (CONT L)) ->
+                   P (ig_msg ST FROM TO CONT)))
+  : forall G, P G.
+Proof.
+  fix Ih 1; case.
+  - by apply: P_end.
+  - move=> ST F T C; apply: P_msg => L.
+    case: (C L)=>[[Ty G]|].
+    + by rewrite /P_option/P_prod; apply/Ih.
+    + by rewrite /P_option.
+Qed.
+
+Lemma ig_ty_ind
+      (P : ig_ty -> Prop)
+      (P_end : forall CONT, P (ig_end CONT))
+      (P_msg : (forall ST FROM TO CONT,
+                   (forall L Ty G, CONT L = Some (Ty, G) -> P G) ->
+                   P (ig_msg ST FROM TO CONT)))
+  : forall G, P G.
+Proof.
+  elim/ig_ty_ind'=>// ST FROM TO CONT Ih.
+  apply/P_msg => L Ty G; move: (Ih L); case: (CONT L) =>[[Ty' G']|]//=.
+  by move=> P_G' [_ <-].
+Qed.
+
+Lemma ig_ty_rect'
+      (P : ig_ty -> Type)
+      (P_end : forall CONT, P (ig_end CONT))
+      (P_msg : (forall ST FROM TO CONT,
+                   (forall L, P_option (P_prod P) (CONT L)) ->
+                   P (ig_msg ST FROM TO CONT)))
+  : forall G, P G.
+Proof.
+  fix Ih 1; case.
+  - by apply: P_end.
+  - move=> ST F T C; apply: P_msg => L.
+    case: (C L)=>[[Ty G]|].
+    + by rewrite /P_option/P_prod; apply/Ih.
+    + by rewrite /P_option.
+Qed.
+
+Lemma ig_ty_rect
+      (P : ig_ty -> Type)
+      (P_end : forall CONT, P (ig_end CONT))
+      (P_msg : (forall ST FROM TO CONT,
+                   (forall L Ty G, CONT L = Some (Ty, G) -> P G) ->
+                   P (ig_msg ST FROM TO CONT)))
+  : forall G, P G.
+Proof.
+  elim/ig_ty_rect'=>// ST FROM TO CONT Ih.
+  apply/P_msg => L Ty G; move: (Ih L); case: (CONT L) =>[[Ty' G']|]//=.
+  by move=> P_G' [_ <-].
+Qed.
+
+Inductive part_of: role -> rg_ty -> Prop :=
+  | pof_from F T C: part_of F (rg_msg F T C)
+  | pof_to F T C: part_of T (rg_msg F T C)
+  | pof_cont p F T C L G Ty: C L = Some (Ty, G)
+    -> part_of p G -> part_of p (rg_msg F T C).
+
+Inductive part_of_all: role -> rg_ty -> Prop :=
+  | pall_from F T C: part_of_all F (rg_msg F T C)
+  | pall_to F T C: part_of_all T (rg_msg F T C)
+  | pall_cont p F T C :
+      P_all (part_of_all p) C -> part_of_all p (rg_msg F T C).
+
+(* Needed to build the next global type in a step  *)
+Inductive part_of_allT: role -> rg_ty -> Type :=
+  | pallT_from F T C: part_of_allT F (rg_msg F T C)
+  | pallT_to F T C: part_of_allT T (rg_msg F T C)
+  | pallT_cont p F T C :
+      (forall l Ty G, C l = Some (Ty, G) -> part_of_allT p G) ->
+      part_of_allT p (rg_msg F T C).
+
+Inductive iPart_of: role -> ig_ty -> Prop :=
+  | ipof_end p cG: part_of p cG -> iPart_of p (ig_end cG)
+  | ipof_from F T C: iPart_of F (ig_msg None F T C)
+  | ipof_to o F T C: iPart_of T (ig_msg o F T C)
+  | ipof_cont p o F T C L G Ty: C L = Some (Ty, G)
+    -> iPart_of p G -> iPart_of p (ig_msg o F T C).
+
+Lemma rgend_part p G : part_of_all p G -> G = rg_end -> False.
+Proof. by move=>[]. Qed.
+
+Lemma pall_inv F T C G p :
+  part_of_all p G -> G = rg_msg F T C -> F <> p -> T <> p ->
+  (forall l Ty G, C l = Some (Ty, G) -> part_of_all p G).
+Proof.
+    by move=>[ F' T' C' [->]//
+             | F' T' C' [_ ->]//
+             |{}p F' T' C' ALL [_ _ <-] _ _ l Ty {}G /ALL
+             ].
+Defined.
+
+Fixpoint find_partsc p G (H : part_of_all p G) {struct H}
+  : part_of_allT p G
+  :=
+  match G as G0 return G = G0 -> part_of_allT p G0 with
+  | rg_msg F T C => fun EQ =>
+                      match @eqP role F p with
+                      | ReflectT pF => match EQ, pF with
+                                       | erefl, erefl => pallT_from F T C
+                                       end
+                      | ReflectF pF =>
+                        match @eqP role T p with
+                        | ReflectT pT => match EQ, pT with
+                                         | erefl, erefl => pallT_to F T C
+                                         end
+                        | ReflectF pT =>
+                          pallT_cont F T
+                                     (fun l Ty G Cl =>
+                                        find_partsc (pall_inv H EQ pF pT Cl))
+                        end
+                      end
+  | rg_end => fun E => match rgend_part H E with end
+  end erefl.
+
+Definition rg_unr (G : rg_ty) : ig_ty :=
+  match G with
+  | rg_msg F T C
+      => ig_msg None F T
+                (fun lbl =>
+                  match C lbl with
+                  | None => None
+                  | Some (t, G) => Some (t, ig_end G)
+                  end)
+  | rg_end => ig_end rg_end
+  end.
