theories/Global/Unravel.v
@@ -1,0 +1,183 @@
+From mathcomp.ssreflect Require Import all_ssreflect seq.
+From mathcomp Require Import finmap.
+
+From Paco Require Import paco paco2.
+
+Set Implicit Arguments.
+Unset Strict Implicit.
+Import Prenex Implicits.
+
+Require Import MPST.Common.
+
+Require Import MPST.Global.Syntax.
+Require Import MPST.Global.Tree.
+
+
+Definition grel := g_ty -> rg_ty -> Prop.
+Inductive g_unroll (r : grel) : grel :=
+| gu_end :
+    g_unroll r g_end rg_end
+| gu_rec IG CG :
+    r (g_open 0 (g_rec IG) IG) CG ->
+    g_unroll r (g_rec IG) CG
+| gu_msg FROM TO iCONT cCONT :
+    same_dom (find_cont iCONT) cCONT ->
+    R_all r (find_cont iCONT) cCONT ->
+    g_unroll r (g_msg FROM TO iCONT) (rg_msg FROM TO cCONT).
+Definition GUnroll IG CG : Prop := paco2 g_unroll bot2 IG CG.
+
+Derive Inversion gunr_inv with (forall r G cG, g_unroll r G cG) Sort Prop.
+Hint Constructors g_unroll.
+
+Lemma gunroll_monotone : monotone2 g_unroll.
+Proof.
+  move=> IG CG r r' U H; move: IG CG U.
+  elim=>[|V|G IH|F T C IH] CG;
+    case E:_ _/ =>[|G' CG' R|F' T' C' CC DOM U]//.
+  - by move: E R=>[<-]{G'} /H; constructor.
+  - by constructor=>// l Ty IG {}CG H0 H1; apply/H/(U _ _ _ _ H0 H1).
+Qed.
+Hint Resolve gunroll_monotone.
+
+Lemma gunroll_unfold r iG cG
+  : paco2 g_unroll r iG cG -> @g_unroll (upaco2 g_unroll r) iG cG.
+Proof. by move/(paco2_unfold gunroll_monotone). Qed.
+
+Lemma g_unroll_rec (r : grel) n iG cG :
+  (forall n IG CG, r IG CG -> paco2 g_unroll r (n_unroll n IG) CG) ->
+  paco2 g_unroll r iG cG <-> paco2 g_unroll r (n_unroll n iG) cG.
+Proof.
+  move=> H; split.
+  - elim: n =>// n Ih in iG cG *.
+    move=> /gunroll_unfold-[]//=.
+    + by apply/paco2_fold.
+    + by move=>IG CG  [/Ih//|/H].
+    + by move=>F T IC CC DOM UA; apply/paco2_fold; constructor.
+  - elim: n =>// n Ih in iG cG *.
+    by case: iG=>//= G H1; apply/paco2_fold; constructor; left; apply/Ih.
+Qed.
+
+Lemma GUnroll_ind n iG cG :
+  GUnroll iG cG <-> GUnroll (n_unroll n iG) cG.
+Proof. by apply/g_unroll_rec. Qed.
+
+Lemma gen2 A B (x' : A) (y' : B) Q P :
+  (forall x y, Q x y -> x = x' -> y = y' -> P) ->
+  Q x' y' -> P.
+Proof. by move=>H /H/( _ erefl erefl).  Qed.
+
+Lemma r_in_unroll_msg r G p q Ks :
+  GUnroll G (rg_msg p q Ks) ->
+  guarded 0 G ->
+  g_closed G ->
+  (r == p) || (r == q) ->
+  r \in participants G.
+Proof.
+  move=> GU GG CG r_pq; apply/(r_in_unroll_rec_depth).
+  move: (unroll_guarded CG GG) r_pq => H.
+  move: GU=>/(GUnroll_ind (rec_depth G)); move: H.
+  move: (n_unroll _ G) => [|v|G'|p' q' Ks'].
+  - by move=>_; apply: gen2=>iG cG /gunroll_unfold-[].
+  - by move=>_; apply: gen2=>iG cG /gunroll_unfold-[].
+  - by move=>/(_ G')/eqP.
+  - move=>_; apply: gen2=>iG cG /gunroll_unfold-[]//.
+    move=>F T IC CC DOM ALL E1 E2; move: E1 E2 DOM ALL=>[->->->][->->->].
+    by move=>_ _; rewrite !in_cons orbA=>->.
+Qed.
+
+Lemma g_closed_unroll n iG : g_closed iG -> g_closed (n_unroll n iG).
+Proof. by elim: n iG=>[|n Ih]//=; case=>//= iG /gopen_closed/Ih. Qed.
+
+
+Lemma g_guarded_unroll iG :
+  g_closed (g_rec iG) -> guarded 0 (g_rec iG) -> guarded 0 (unroll iG).
+Proof.
+  move=> C GG; have GG': (guarded 1 iG) by move:GG C=>/=; case: iG.
+  move: (guarded_open 0 GG C GG')=>/guarded_depth_gt.
+  by move=>/(_ _ _ (leq0n 1) (gopen_closed C)).
+Qed.
+
+Lemma g_guarded_nunroll n iG
+  : g_closed iG -> guarded 0 iG -> guarded 0 (n_unroll n iG).
+Proof.
+  elim: n iG=>[|n Ih]//;case=>// iG CG /(g_guarded_unroll CG)/Ih-H/=.
+  by apply/H/gopen_closed.
+Qed.
+
+CoFixpoint g_expand (g : g_ty) : rg_ty :=
+  match n_unroll (rec_depth g) g with
+  | g_msg F T Ks =>
+    rg_msg F T
+           (fun l =>
+              match find_cont Ks l with
+              | Some (Ty, G) => Some (Ty, g_expand G)
+              | None => None
+              end)
+  | _ => rg_end
+  end.
+
+Lemma rgtyU G : G = match G with
+                    | rg_msg F T C => rg_msg F T C
+                    | rg_end => rg_end
+                    end.
+Proof. by case: G. Qed.
+
+Definition g_expand' G :=
+  match G with
+  | g_msg F T Ks =>
+    rg_msg F T (fun l : lbl => match find_cont Ks l with
+                               | Some (Ty, G0) => Some (Ty, g_expand G0)
+                               | None => None
+                               end)
+  | _ => rg_end
+  end.
+
+Lemma g_expand_once G : g_expand G = g_expand' (n_unroll (rec_depth G) G).
+Proof.
+  by rewrite (rgtyU (g_expand _)) /g_expand /g_expand'-rgtyU-/g_expand.
+Qed.
+
+Lemma g_expand_unr G :
+  guarded 0 G ->
+  g_closed G ->
+  non_empty_cont G ->
+  GUnroll G (g_expand G).
+Proof.
+  move=>gG cG NE; rewrite g_expand_once.
+  move: {-1}(g_expand' _) (erefl (g_expand' (n_unroll (rec_depth G) G))).
+  move=>CG ECG; move: G CG {ECG gG cG NE}(conj ECG (conj gG (conj cG NE))).
+  apply/paco2_acc=>r _ /(_ _ _ (conj erefl (conj _ (conj _ _))))-CIH.
+  move=> G CG [<-]{CG} [gG][cG][NE].
+  case: G cG gG NE.
+  - move=>_ _ _ /=; by apply/paco2_fold; constructor.
+  - by move=>V /closed_not_var/(_ V)/eqP/(_ erefl).
+  - move=>G cG gG nE /=;apply/paco2_fold.
+    constructor; right; have gG': guarded 1 G by move: gG.
+    rewrite (guarded_recdepth (m:=0) gG' _ (g_rec G)) //.
+    apply/CIH.
+    by apply/g_guarded_unroll.
+    by apply/gopen_closed.
+    by apply/ne_open.
+  - move=>F T C cG gG NE; apply/paco2_fold; constructor.
+    + move=>l Ty; case: find_cont=>[[Ty0 L0]|]//; split=>[][G]//[->] _.
+      * by exists (g_expand L0).
+      * by exists L0.
+    + move=> l Ty G CG FND; rewrite FND=>[][<-]; right.
+      move: cG; rewrite /g_closed/==>/flatten_eq_nil/member_map-cG.
+      move: gG; rewrite /==>/forallbP/forall_member-gG.
+      move: NE=>/==>/andP-[NE_C]/forallbP/forall_member/member_map-NE.
+      move: (find_member FND)=>MEM.
+      rewrite g_expand_once.
+      by apply/(CIH _ (gG _ MEM) (cG _ MEM) (NE _ MEM)).
+Qed.
+
+Lemma expand_g_end g
+      : is_end g -> g_expand g = rg_end.
+Proof.
+  rewrite (rgtyU (g_expand _))/=.
+  suff: is_end g -> n_unroll (rec_depth g) g = g_end by move=>E /E->.
+  move: {-1}(rec_depth g) (erefl (rec_depth g))=> n.
+  elim: n g; first by case=>//.
+  move=>n Ih; case=>//= g [] RD END; move: (recdepth_unroll END) RD=>->{}RD.
+  by move: END=>/isend_unroll; apply/Ih.
+Qed.
