theories/Local/Semantics.v
@@ -1,0 +1,248 @@
+From mathcomp.ssreflect Require Import all_ssreflect seq.
+From mathcomp Require Import finmap.
+
+From Paco Require Import paco paco2.
+Set Implicit Arguments.
+Unset Strict Implicit.
+Import Prenex Implicits.
+
+Require Import MPST.Common.
+
+Require Import MPST.Local.Syntax.
+Require Import MPST.Local.Tree.
+Require Import MPST.Local.Unravel.
+
+Notation renv := {fmap role -> rl_ty}.
+Notation qenv := {fmap role * role -> seq (lbl * mty) }.
+
+Definition enq (qs : {fmap (role * role) -> (seq (lbl * mty))}) k v :=
+  match qs.[? k] with
+  | Some vs => qs.[ k <- app vs [:: v] ]
+  | None => qs.[ k <- [:: v]]
+  end%fmap.
+
+Definition deq (qs : {fmap (role * role) -> (seq (lbl * mty))}) k :=
+  match qs.[? k] with
+  | Some vs =>
+    match vs with
+    | v :: vs => if vs == [::] then Some (v, qs.[~ k])
+                 else Some (v, qs.[k <- vs])
+    | [::] => None
+    end
+  | None => None
+  end%fmap.
+
+Definition look (E : {fmap role -> rl_ty}) p := odflt rl_end E.[? p]%fmap.
+
+Definition do_act_lt (L : rl_ty) A :=
+let: (mk_act a p q l t) := A in
+match L with
+| rl_msg a' q' Ks =>
+  match Ks l with
+  | Some (t', Lp) =>
+    if (a == a') && (q == q') && (t == t')
+    then Some Lp
+    else None
+  | None => None
+  end
+| _ => None
+end%fmap.
+
+Definition run_act_lt (L : rl_ty) A := odflt L (do_act_lt L A).
+
+Definition do_act (P : renv) A :=
+  let: (mk_act a p q l t) := A in
+  match do_act_lt (look P p) A with
+  | Some Lp => Some (P.[p <- Lp]%fmap)
+  | None => None
+  end.
+
+Lemma doact_send (E : renv) p q lb t KsL Lp :
+  (look E p = rl_msg l_send q KsL) ->
+  (KsL lb = Some (t, Lp)) ->
+  exists E', (do_act E (mk_act l_send p q lb t) = Some E').
+Proof.
+  move=>H1 H2; rewrite /do_act/do_act_lt H1 H2 !eq_refl/=.
+  by exists E.[ p <- Lp]%fmap.
+Qed.
+
+Definition do_act_l_ty (L: l_ty) (A : act) : option l_ty :=
+  let: (mk_act a p q l t) := A in
+  match lunroll (lrec_depth L) L with
+  | l_msg a' q' Ks =>
+    match find_cont Ks l with
+    | Some (t', Lp) =>
+      if (a == a') && (q == q') && (t == t')
+      then Some Lp
+      else None
+    | None => None
+    end
+  | _ => None
+  end.
+
+Definition run_act_l_ty (L: l_ty) (A : act) : l_ty := odflt L (do_act_l_ty L A).
+
+Lemma do_act_works Li Lr A :
+  LUnroll Li Lr -> LUnroll (run_act_l_ty Li A) (run_act_lt Lr A).
+Proof.
+  rewrite /run_act_l_ty/run_act_lt/do_act_l_ty/do_act_lt/==>LU.
+  case: A=> a _ q l t; move: ((LUnroll_ind (lrec_depth Li) Li Lr).1 LU)=>LU'.
+  move: LU' LU.
+  case EQ: (lunroll (lrec_depth Li) Li)=> [| v | Li' | a' p C].
+  - by move=> /lunroll_end->.
+  - by move=>/(paco2_unfold l_unroll_monotone); case F: _ _ /.
+  - by move=>/= _ _; apply/(lunroll_inf _ EQ).
+  - move=>/(paco2_unfold l_unroll_monotone).
+    case F: _ _ / =>[||a0 p0 K0 C0 DOM UNR]//.
+    move: F DOM UNR=>[<-<-<-] DOM UNR{a0 p0 K0 EQ}.
+    case EQ: find_cont=>[[Ty L]|]//; last by rewrite (dom_none DOM EQ).
+    move: (dom DOM EQ)=>[{}Lr] EQ'; rewrite EQ'/=.
+    case: (boolP ((a == a') && (q == p) && (t == Ty)))=>//= _ _.
+    by move: (UNR _ _ _ _ EQ EQ')=>[].
+Qed.
+
+Open Scope fmap_scope.
+(** lstep a Q P Q' P' is the 'step' relation <P, Q> ->^a <P', Q'> in Coq*)
+Inductive lstep : act -> renv * qenv -> renv * qenv -> Prop :=
+| ls_send t p q lb (P P' : renv) (Q Q' : qenv) :
+    Q' == enq Q (p, q) (lb, t) ->
+    do_act P (mk_act l_send p q lb t) = Some P' ->
+    lstep (mk_act l_send p q lb t) (P, Q) (P', Q')
+| ls_recv t p q lb (P P' : renv) (Q Q' : qenv) :
+    deq Q (p, q) == Some ((lb, t), Q') ->
+    do_act P (mk_act l_recv q p lb t) = Some P' ->
+    lstep (mk_act l_recv q p lb t) (P, Q) (P', Q')
+.
+Derive Inversion lstep_inv with (forall A P P', lstep A P P') Sort Prop.
+
+Definition runnable (A : act) (P : renv * qenv) : bool :=
+  match do_act P.1 A with
+  | Some _ =>
+    let: mk_act a p q l t := A in
+    match a with
+    | l_send => true
+    | l_recv =>
+      match deq P.2 (q, p) with
+      | Some ((l', t'), Q) => (l == l') && (t == t')
+      | None => false
+      end
+    end
+  | None => false
+  end.
+
+Lemma lstep_runnable A P P' : lstep A P P' -> runnable A P.
+Proof.
+  by case=> Ty F T l {P P'}E E' Q Q' /eqP-QFT /=; case LOOK: look=>[|a p C]//;
+     case Cl: (C l)=>[[Ty' L]|]//; case: ifP=>//EQ _;
+     rewrite /runnable/= LOOK Cl EQ // QFT !eq_refl.
+Qed.
+
+Lemma lstep_eq A P P0 P1 : lstep A P P0 -> lstep A P P1 -> P0 = P1.
+Proof.
+  case=>Ty0 F0 T0 l0 {P P0}E E0 Q Q0 /eqP-QFT/=; case LOOK: look=>[|a p C]//;
+  case Cl: (C l0)=>[[Ty' L]|]//; case: ifP=>//EQ [<-];
+  elim/lstep_inv =>// _ Ty1 F1 T1 l1 E' E1 Q' Q1 /eqP-QFT'/= ACT EQ1 EQ2 EQ3;
+  move: EQ1 EQ2 EQ3 ACT QFT QFT'=>[->->->->] [->->] _ {F1 T1 l1 Ty1 E' Q' P1};
+  rewrite LOOK Cl EQ=>[][<-]->.
+  - by move=>->.
+  - by move=>[->].
+Qed.
+
+Definition do_queue (Q : qenv) (A : act) : qenv :=
+  match A with
+  | mk_act l_send F T l Ty => enq Q (F, T) (l, Ty)
+  | mk_act l_recv F T l Ty =>
+    match deq Q (T, F) with
+    | Some (_, Q') => Q'
+    | None => Q
+    end
+  end.
+
+(* Attempts to run a step, does nothing if it cannot run *)
+Definition run_step (A : act) (P : renv * qenv) : renv * qenv :=
+  match do_act P.1 A with
+  | Some E' => (E', do_queue P.2 A)
+  | _ => P
+  end.
+
+(* Lemma run_step 'makes sense' *)
+Lemma run_step_sound A P : runnable A P -> lstep A P (run_step A P).
+Proof.
+  case: P => E Q.
+  rewrite /runnable /=; case E_doact: (do_act _ _)=>[E'|//].
+  case: A E_doact=> [[|] p q l t E_doact]/=.
+  - by move=> _; rewrite /run_step E_doact; constructor=>//.
+  - case E_deq: (deq _ _) =>[[[l' t'] Q']|//].
+    case: (boolP ((l == l') && _)) =>[/andP-[/eqP-ll' /eqP-tt']|//] _.
+    move: ll' tt' E_deq =><-<- E_deq.
+    rewrite /run_step E_doact /= E_deq.
+      by constructor =>//; first by apply/eqP.
+Qed.
+
+Lemma run_step_compl A P P' : lstep A P P' -> P' = run_step A P.
+Proof.
+  by move=> ST; move: (lstep_runnable ST)=>/run_step_sound/(lstep_eq ST).
+Qed.
+
+Definition rel_trc := trace act -> renv*qenv -> Prop.
+Inductive l_lts_ (r : rel_trc) : rel_trc :=
+| lt_end E :
+    (forall p, look E p = rl_end) ->
+    @l_lts_ r (tr_end _) (E, [fmap])
+| lt_next a t P P' :
+    lstep a P P' ->
+    r t P' ->
+    @l_lts_ r (tr_next a t) P.
+Hint Constructors l_lts_.
+Lemma l_lts_monotone : monotone2 l_lts_.
+Proof. pmonauto. Qed.
+Hint Resolve l_lts_monotone : paco.
+
+Definition l_lts t L := paco2 l_lts_ bot2 t L.
+Derive Inversion llts_inv with (forall tr G, l_lts tr G) Sort Prop.
+
+Definition rty_trc := trace act -> rl_ty -> Prop.
+Inductive l_trc_ (p : role) (r : rty_trc) : rty_trc :=
+| l_trc_end : l_trc_ p r (tr_end _) rl_end
+| l_trc_msg A TR L L' :
+    subject A == p -> do_act_lt L A = Some L' ->
+    r TR L' ->
+    l_trc_ p r (tr_next A TR) L
+.
+Lemma l_trc_monotone p : monotone2 (l_trc_ p).
+Proof.
+  move=>TR cL r r' Htrc MON; move: Htrc; case.
+  - by constructor.
+  - move=>A TR0 L L' Hsubj Hact /MON.
+    by move: Hsubj Hact; apply l_trc_msg.
+Qed.
+
+Definition l_trc p t L := paco2 (l_trc_ p) bot2 t L.
+
+Definition trc_rel := trace act -> trace act -> Prop.
+Inductive subtrace_ (p : role) (r : trc_rel) : trc_rel :=
+| subtrace_end : subtrace_ p r (tr_end _) (tr_end _)
+| subtrace_skip A TRp TR :
+    subject A != p ->
+    r TRp TR ->
+    subtrace_ p r TRp (tr_next A TR)
+| subtrace_msg A TRp TR :
+    subject A == p ->
+    r TRp TR ->
+    subtrace_ p r (tr_next A TRp) (tr_next A TR)
+.
+Lemma subtrace_monotone p : monotone2 (subtrace_ p).
+Proof.
+  move=>TR cL r r' Htrc MON; move: Htrc; case.
+  - by constructor.
+  - move=> A TRp TR0 Hsubj /MON; move: Hsubj.
+    by apply: subtrace_skip.
+  - move=> A TRp TR0 Hsubj /MON; move: Hsubj.
+    by apply: subtrace_msg.
+Qed.
+Definition subtrace p T0 T1 := paco2 (subtrace_ p) bot2 T0 T1.
+Hint Constructors EqL_.
+Hint Resolve EqL_monotone.
+Hint Resolve EqL_refl.
+
+Notation cfg := (renv * qenv)%type.
