theories/Local/Syntax.v
@@ -1,0 +1,532 @@
+From mathcomp.ssreflect Require Import all_ssreflect seq.
+From mathcomp Require Import finmap.
+
+From Paco Require Import paco paco2.
+Set Implicit Arguments.
+Unset Strict Implicit.
+Import Prenex Implicits.
+
+Require Import MPST.Common.
+
+Unset Elimination Schemes.
+Inductive l_ty :=
+| l_end
+| l_var (v : nat)
+| l_rec (L : l_ty)
+| l_msg (a : l_act) (r : role) (Ks : seq (lbl * (mty * l_ty)))
+.
+Set Elimination Schemes.
+
+Definition ilook (E : seq (role * l_ty)) p := odflt l_end (find_cont E p).
+
+Fixpoint partsL (G : l_ty) :=
+  match G with
+  | l_end
+  | l_var _ => [::]
+  | l_rec G => partsL G
+  | l_msg a p Ks => p::flatten [seq partsL K.2.2 | K <- Ks]
+  end.
+
+Lemma lty_ind :
+  forall (P : l_ty -> Prop),
+    P l_end ->
+    (forall v, P (l_var v)) ->
+    (forall G, P G -> P (l_rec G)) ->
+    (forall a p Ks, Forall (fun K => P K.2.2) Ks -> P (l_msg a p Ks)) ->
+    forall l : l_ty, P l.
+Proof.
+  move => P P_end P_var P_rec P_msg.
+  fix Ih 1; case=>[|v|L|a r K].
+  + by apply: P_end.
+  + by apply: P_var.
+  + by apply: P_rec.
+  + by apply: P_msg; elim: K.
+Qed.
+
+Fixpoint depth_lty L :=
+  match L with
+  | l_end
+  | l_var _ => 0
+  | l_rec L => (depth_lty L).+1
+  | l_msg _ _ Ks => (foldr maxn 0 [seq depth_lty K.2.2 | K <- Ks]).+1
+  end.
+
+Fixpoint eq_lty x y :=
+  match x, y with
+  | l_end, l_end => true
+  | l_var x, l_var y => x == y
+  | l_rec x, l_rec y => eq_lty x y
+  | l_msg a1 r1 Ks1, l_msg a2 r2 Ks2
+    => (a1 == a2) && (r1 == r2)
+         && (fix eqK Ks1 Ks2 :=
+               match Ks1, Ks2 with
+               | [::], [::] => true
+               | K1::Ks1, K2::Ks2 =>
+                 (K1.1 == K2.1)
+                   && (K1.2.1 == K2.2.1)
+                   && eq_lty K1.2.2 K2.2.2
+                   && eqK Ks1 Ks2
+               | _, _ => false
+               end) Ks1 Ks2
+  | _, _ => false
+  end.
+
+Definition eq_lalt (l r : lbl * (mty * l_ty)) :=
+  (l.1 == r.1) && (l.2.1 == r.2.1) && eq_lty l.2.2 r.2.2.
+
+Lemma eqmsg_all a1 a2 r1 r2 K1 K2 :
+  eq_lty (l_msg a1 r1 K1) (l_msg a2 r2 K2) =
+  (a1 == a2) && (r1 == r2) && all2 eq_lalt K1 K2.
+Proof.
+  rewrite /=; do 2 (case: eqP=>///= _); move: K1 K2 {r1 r2 a1 a2}.
+Qed.
+
+Lemma lty_eqP : Equality.axiom eq_lty.
+Proof.
+  rewrite /Equality.axiom; fix Ih 1 => x y.
+  case: x => [|v|L|a r K]; case: y =>[|v'|L'|a' r' K']; try (by constructor).
+  + by rewrite /eq_lty; case: eqP=>[->|F]; constructor=>//[[/F]].
+  + by rewrite /=; case: Ih=>[->|F]; constructor=>//[[/F]].
+  + rewrite eqmsg_all; do 2 (case: eqP=>[<-|F]/=;[|constructor=>[[/F]]//]).
+    elim: K K'=>[|[l [t L]] K IhK];
+      case=>[|[l' [t' L']]K']/=; try (by constructor).
+    rewrite {1}/eq_lalt/=; do 2 (case: eqP=>[<-|F];[|constructor=>[[/F]]//]).
+    case: Ih=>[<-|F];[|constructor=>[[/F]]//].
+    by case: IhK=>[[]<-|F]; constructor=>//[[]]H; apply: F; rewrite H.
+Qed.
+
+Definition lty_eqMixin := EqMixin lty_eqP.
+Canonical lty_eqType := Eval hnf in EqType l_ty lty_eqMixin.
+
+Lemma in_maximum_leq v l: v \in l -> v <= foldr maxn 0 l.
+Proof.
+  elim: l=>//v' l Ih; rewrite in_cons=>/orP-[/eqP<-|]/=.
+  + by apply: leq_maxl.
+  + by move=>/Ih{Ih}; move: (foldr _ _ _) => k {l}; rewrite leq_max orbC=>->.
+Qed.
+
+Lemma l_ty_ind :
+  forall (P : l_ty -> Prop),
+    P l_end ->
+    (forall v, P (l_var v)) ->
+    (forall L, P L -> P (l_rec L)) ->
+    (forall a p Ks, (forall K, K \in Ks -> P K.2.2) -> P (l_msg a p Ks)) ->
+    forall l : l_ty, P l.
+Proof.
+  move => P P_end P_var P_rec P_msg L.
+  move: {-1}(depth_lty L) (leqnn (depth_lty L))=> n; move: n L; elim.
+  + by case.
+  + move=>n Ih; case=>/=//.
+  - by move=>L D; apply:P_rec; apply: Ih.
+  - move=> a r Ks D;apply: P_msg=>K /(map_f (fun X => depth_lty X.2.2)).
+    move=>/in_maximum_leq-/=dG; move: (leq_trans dG D)=>{dG} {D}.
+      by apply: Ih.
+Qed.
+
+Fixpoint l_shift n d (L : l_ty) :=
+  match L with
+  | l_end => l_end
+  | l_var v => if v >= d then l_var (n + v) else L
+  | l_msg a p Ks => l_msg a p [seq (K.1, (K.2.1, l_shift n d K.2.2)) | K <- Ks]
+  | l_rec L => l_rec (l_shift n d.+1 L)
+  end.
+
+Fixpoint l_open (d : nat) (L2 : l_ty) (L1 : l_ty) :=
+  match L1 with
+  | l_end => L1
+  | l_var v => if v == d then l_shift d 0 L2 else L1
+  | l_rec L => l_rec (l_open d.+1 L2 L)
+  | l_msg a p Ks =>
+    l_msg a p [seq (K.1, (K.2.1, l_open d L2 K.2.2)) | K <- Ks]
+  end.
+Notation "{ k '~>' v } L":= (l_open k v L) (at level 30, right associativity).
+Notation "L '^' v":= (l_open 0 (l_var v) L) (at level 30, right associativity).
+
+Lemma open_notvar n L L' :
+  (forall v : nat, L != l_var v) ->
+  (forall v : nat, l_open n L' L != l_var v).
+Proof. by case: L=>//v /(_ v)/eqP. Qed.
+
+Lemma l_open_msg_rw d L2 a r Ks:
+ l_open d L2 (l_msg a r Ks)
+ = l_msg a r [seq (K.1, (K.2.1, l_open d L2 K.2.2)) | K <- Ks].
+Proof. by []. Qed.
+
+Lemma unzip2_lift A B C (f : B -> C) (K : seq (A * B)) :
+  [seq f x | x <- unzip2 K] = unzip2 [seq (x.1, f x.2) | x <- K].
+Proof. by rewrite /unzip2 -!map_comp /comp. Qed.
+
+Lemma unzip1_map2 A B C (f : B -> C) (K : seq (A * B)) :
+  unzip1 K = unzip1 [seq (x.1, f x.2) | x <- K].
+Proof. by rewrite /unzip1 -map_comp /comp. Qed.
+
+Lemma map2_zip A B C (f : B -> C) (K : seq (A * B)) :
+  zip (unzip1 K) [seq f x | x <- unzip2 K] = [seq (x.1, f x.2) | x <- K].
+Proof. by rewrite unzip2_lift (unzip1_map2 f) zip_unzip. Qed.
+
+Fixpoint l_fidx (d : nat) (L : l_ty) : seq nat :=
+  match L with
+  | l_end => [::]
+  | l_var v => if v >= d then [:: v - d] else [::]
+  | l_rec L => l_fidx d.+1 L
+  | l_msg _ _ K => flatten [seq l_fidx d lL.2.2 | lL <- K]
+  end.
+
+Definition l_closed (L : l_ty) := l_fidx 0 L == [::].
+
+Lemma lfbvar_next n G :
+  l_fidx n G == [::] ->
+  l_fidx n.+1 G = [::].
+Proof.
+  elim: G n=>[//|v|G Ih|p q Ks Ih] n/=.
+  - case: v=>//= m H; case: ifP=>// n_m; move: H.
+    by move: (leq_trans (leqnSn n) n_m)=>->.
+  - by apply: Ih.
+  - rewrite flatten_eq_nil member_map=>H; apply/eqP.
+    rewrite flatten_eq_nil member_map=> K /memberP-M.
+    by move: M (Ih K M n)=>/memberP-M /(_ (H K M))=>->.
+Qed.
+
+Lemma lfbvar_gt n m G :
+  n <= m ->
+  l_fidx n G == fset0 ->
+  l_fidx m G = fset0.
+Proof.
+  move=> LE H; move: LE; elim: m=>[|m Ih]//; first by case: n H=>///eqP.
+  move: H; case: (boolP (n == m.+1))=>[/eqP->/eqP//|NE _ LE].
+  apply/lfbvar_next/eqP/Ih; move: (conj NE LE)=>/andP.
+  by rewrite -ltn_neqAle.
+Qed.
+
+Lemma lshift_closed n d G :
+  l_fidx d G == fset0 ->
+  l_shift n d G = G.
+Proof.
+  elim: G=> [| v | L Ih | a p Ks Ih]//= in d *.
+  { (* var *)
+    by case: ifP=>//.
+  }
+  { (* rec *)
+    by move=>H; congr l_rec; apply/Ih.
+  }
+  { (* msg *)
+    move=>/flatten_eq_nil/member_map/(_ _ ((rwP (memberP _ _)).2 _))-H.
+    congr l_msg; rewrite -{2}(map_id Ks); apply/eq_in_map=>K IN.
+    by rewrite (Ih _ IN _ (H _ IN)) -!surjective_pairing.
+  }
+Qed.
+
+Lemma lopen_closed G :
+  l_closed (l_rec G) ->
+  l_closed (l_open 0 (l_rec G) G).
+Proof.
+  rewrite/l_closed/==>G_fbv.
+  have: l_fidx 0 (l_rec G) == fset0 by [].
+  move: (l_rec G) => G' G'0.
+  elim: G 0 G_fbv=>[//|v|G Ih|p q Ks Ih] n /=.
+  - move=> H; case: ifP=>[|/=].
+    + move=> _; rewrite (lshift_closed n G'0); apply/eqP.
+      by move: G'0; apply/lfbvar_gt.
+    + case: ifP=>// LE /(rwP negPf)-NE; move: (conj NE LE)=>/andP.
+      by rewrite eq_sym -ltn_neqAle=>LT; move: H; rewrite LT.
+  - by apply: (Ih n.+1); rewrite lfbvar_next.
+  - rewrite -map_comp/comp/=; move=>/flatten_eq_nil/member_map-H.
+    apply/flatten_eq_nil/member_map=>K /memberP-M.
+    by apply: Ih=>//; apply: H; apply/memberP.
+Qed.
+
+Fixpoint lguarded d L :=
+  match L with
+  | l_end => true
+  | l_var v => v >= d
+  | l_rec L => lguarded d.+1 L
+  | l_msg _ _ Ks => all (fun K => lguarded 0 K.2.2) Ks
+  end.
+
+Fixpoint l_binds n L :=
+  match L with
+  | l_var v => v == n
+  | l_rec L => l_binds n.+1 L
+  | _ => false
+  end.
+
+Fixpoint lguarded' L :=
+  match L with
+  | l_end
+  | l_var _ => true
+  | l_rec L => ~~ l_binds 0 L && lguarded' L
+  | l_msg _ _ Ks => all (fun K => lguarded' K.2.2) Ks
+  end.
+
+Lemma lguarded_next n G : lguarded n.+1 G = ~~ l_binds n G && lguarded n G.
+Proof. by elim: G n=>//= v n; rewrite ltn_neqAle eq_sym. Qed.
+
+Lemma lguarded_binds G : lguarded 0 G = lguarded' G.
+Proof.
+  elim: G=>[||G|_ _ Ks Ih]//=; first by move=><-;apply/lguarded_next.
+  elim: Ks Ih=>[//|K Ks Ih']/= Ih; rewrite Ih ?in_cons ?eq_refl //.
+  by rewrite Ih' // => K' H; apply/Ih; rewrite in_cons orbC H.
+Qed.
+
+Lemma lguarded_rec d L
+  : lguarded d (l_rec L) -> forall s, s <= d -> ~~ l_binds s L.
+elim: L=>[|v|L /= Ih|a p Ks Ih]// in d *.
+- move=>/= vd s sd; move: (leq_ltn_trans sd vd).
+  by rewrite eq_sym ltn_neqAle=>/andP-[].
+- by rewrite /==>/Ih-{Ih}Ih s Lsd; apply/Ih.
+Qed.
+
+Fixpoint lrec_depth L :=
+  match L with
+  | l_rec G => (lrec_depth G).+1
+  | _ => 0
+  end.
+
+Fixpoint lunroll d G :=
+  match d with
+  | 0 => G
+  | d.+1 =>
+    match G with
+    | l_rec G' => lunroll d (l_open 0 G G')
+    | _ => G
+    end
+  end.
+
+Lemma lguarded_match d G :
+  match G with
+  | l_var v => d < v
+  | _ => lguarded d.+1 G
+  end ->
+  (exists v, (G == l_var v) && (d < v)) \/
+  (forall v, (G != l_var v)) /\ lguarded d.+1 G.
+Proof.
+  case: G=>[|||]//=; try by right.
+  by move=> n Eq; left; exists n; rewrite eq_refl.
+Qed.
+
+Lemma lguarded_recdepth d G m :
+  lguarded d G ->
+  m < d ->
+  forall G', lrec_depth G = lrec_depth ({m ~> G'} G).
+Proof.
+  elim: G=>[|n|G Ih|p q Ks Ih]//= in d m *.
+  - move=>dn md G; case: ifP=>[/eqP-E|ne//].
+    by move: E dn md=>-> /leq_ltn_trans-H /H; rewrite ltnn.
+  - by move=> GG md G'; rewrite (Ih _ m.+1 GG _ G').
+Qed.
+
+Lemma lty_not_var A G (b1 : nat -> A) (b2 : A) :
+  (forall v : nat, G != l_var v) ->
+  match G with | l_var v => b1 v | _ => b2 end = b2.
+Proof. by case: G =>[|n /(_ n)/eqP||]. Qed.
+
+Lemma lguarded_depth_gt dG dG' G :
+  lguarded dG' G -> l_closed G -> lguarded dG G.
+Proof.
+  rewrite /l_closed=> H H'; move: 0 (leq0n dG') H H'.
+  elim: G =>[|n|G Ih|p q Ks Ih]// in dG dG' *.
+  - by move=> m /leq_trans-H /= /H->.
+  - by move=> n ndG' /=; apply/Ih.
+Qed.
+
+Lemma lclosed_not_var G :
+  l_closed G ->
+  forall v, G != l_var v.
+Proof.
+  rewrite /l_closed.
+  by case: G=>//= v.
+Qed.
+
+Lemma lopen_not_var d G G' :
+  l_closed G ->
+  (forall v, G' != l_var v) ->
+  forall v, {d ~> G} G' != l_var v.
+Proof. by case: G'=>// n _ /(_ n)/eqP. Qed.
+
+Lemma lguarded_open d1 d2 G G' :
+  lguarded 0 G' ->
+  l_closed G' ->
+  lguarded d1 G ->
+  lguarded d1 ({d2 ~> G'} G).
+Proof.
+  elim: G=>[|n|G Ih|p q Ks Ih]//= in d1 d2 *.
+  - case: ifP=>// _ gG cG; rewrite (lshift_closed _ cG)=>_.
+    by apply/(lguarded_depth_gt _ gG).
+  - by apply/Ih.
+  - move=> GG' CG'; elim: Ks=>[|K Ks IhK]//= in Ih *.
+    move: (Ih K); rewrite in_cons eq_refl=>/(_ is_true_true _ _ GG' CG')-H.
+    move=>/andP-[GK GKs]; move: H=>/(_ _ _ GK)->//=.
+    by apply/IhK=>// K0 MK0; apply/Ih; rewrite in_cons orbC MK0.
+Qed.
+
+Lemma lguarded_gt d d' G :
+  d >= d' ->
+  lguarded d G ->
+  lguarded d' G.
+Proof.
+  elim: G=>[|n|G Ih|p q Ks Ih]//= in d d' *.
+  - by move=>/leq_trans-H /H.
+  - by move=> H; apply/Ih.
+Qed.
+
+Lemma lunroll_guarded G :
+  l_closed G ->
+  lguarded 0 G ->
+  forall G', lunroll (lrec_depth G) G != l_rec G'.
+Proof.
+  move: {-2}(lrec_depth G) (eq_refl (lrec_depth G)) => n.
+  elim: n => [|n Ih]/= in G *; case: G=>// G n_rd CG GG; move: n_rd.
+  rewrite eqE/=-eqE => n_rd.
+  have/=GG': (lguarded 0 (l_rec G)) by [].
+  move: n_rd; rewrite (lguarded_recdepth GG' (ltn0Sn 0) (l_rec G))=>n_rd.
+  apply/Ih=>//; first by apply/lopen_closed.
+  by apply/lguarded_open=>//; apply/lguarded_gt; last by apply/GG'.
+Qed.
+
+Fixpoint l_isend L {struct L}:=
+  match L with
+  | l_rec L => l_isend L
+  | l_end => true
+  | _ => false
+  end.
+
+Lemma isend_open n L' L :
+  l_isend L -> l_open n L' L = L.
+Proof.
+  elim: L=>[|v|L Ih|a p KS Ih]//= in n *; move=> END.
+  by rewrite Ih.
+Qed.
+
+Lemma keep_unrolling L :
+  l_isend L -> exists m, l_end = lunroll m L.
+Proof.
+  elim: L=>[||L Ih|]//; [move=>_| move=>/=END; move:(Ih END)=>[n U]].
+  - by exists 0.
+  - by exists n.+1=>/=; rewrite (isend_open 0 _ END).
+Qed.
+
+Lemma l_closed_no_binds_aux m n L: m <= n -> l_fidx m L == fset0
+  -> l_binds n L = false.
+Proof.
+elim: L m n; rewrite //=.
++ move=> v m n le; case: ifP=>//.
+  by move=> lefalse; elim; apply: ltn_eqF;
+    apply: (leq_trans _ le); move: (negbT lefalse); rewrite-ltnNge //=.
++ by move=> L IH m n le; apply: IH; rewrite //=.
+Qed.
+
+Lemma l_closed_no_binds n L: l_closed L -> l_binds n L = false.
+Proof. by apply: l_closed_no_binds_aux. Qed.
+
+Lemma l_binds_open m n L L1: n != m -> l_closed L1
+  -> l_binds m (l_open n L1 L) = l_binds m L.
+Proof.
+elim: L m n L1.
++ by move=> m n L1 neq closed; rewrite /l_binds //=.
++ move=> v m n L1 neq closed.
+  rewrite /l_binds //=; case: ifP => //=; rewrite <-(rwP eqP); move=>->.
+  rewrite (lshift_closed _ closed).
+  move: (@l_closed_no_binds m _ closed); rewrite /l_binds; move =>->.
+  by move: (negbTE neq).
++ by move=> L IH m n L1 neq closed; rewrite //=; apply: IH.
++ by [].
+Qed.
+
+Fixpoint n_rec d L :=
+  match d with
+  | 0 => L
+  | d.+1 => l_rec (n_rec d L)
+  end.
+
+Fixpoint n_open d n L :=
+  match n with
+  | 0 => L
+  | m.+1 => l_open d (n_rec d.+1 (n_open d.+1 m L)) (n_open d.+1 m L)
+  end.
+
+Fixpoint get_nr L :=
+  match L with
+  | l_rec L => get_nr L
+  | _ => L
+  end.
+
+Lemma nrec_comm d L : n_rec d (l_rec L) = n_rec d.+1 L.
+Proof. by elim: d =>//= n ->. Qed.
+
+Lemma nopen_rec_comm n L : n_open 0 n (l_rec L) = l_rec (n_open 1 n L).
+Proof.
+  elim: n 0 L=>//= n Ih d L.
+  rewrite Ih/= -Ih/= -/(n_rec d.+1 _) -/(n_rec d.+2 _).
+  by rewrite Ih -/(n_rec d.+2 _) nrec_comm.
+Qed.
+
+Lemma lunroll_nopen L :
+  lunroll (lrec_depth L) L = n_open 0 (lrec_depth L) (get_nr L).
+Proof.
+  rewrite -{2}/(n_open 0 0 L) -{2}(@addn0 (lrec_depth L)); move: {2 4}0 => n.
+  elim: L n=>//= L Ih n.
+  rewrite nopen_rec_comm/= -/(n_open 0 (lrec_depth L + n).+1 _).
+  by rewrite -/(n_open 0 n.+1 _); rewrite Ih addnS.
+Qed.
+
+Lemma nopen_var' m n L v : n_open m n L = l_var v -> L = l_var v.
+Proof.
+  elim: n m=>//= n Ih m.
+  case EQ: n_open=>[|v'||]//=; case: ifP=>// _ [EV].
+  by move: EV EQ=>->{v'}/Ih.
+Qed.
+
+Lemma getnr_nonrec L : match get_nr L with
+                       | l_rec _ => false
+                       | _ => true
+                       end.
+Proof. by elim: L. Qed.
+
+(* lbinds m (get_nr L) is the same as get_nr L = l_var m *)
+Lemma nopen_rec d n L L' :
+  n_open d n (get_nr L) = l_rec L' ->
+  exists m, l_binds m (get_nr L) /\ m < d + n.
+Proof.
+  elim: n =>[|n Ih] //= in d L' *;
+    first by move=> H; move: H (getnr_nonrec L)=>->.
+  case EQ: (n_open d.+1 n (get_nr L)) => [|v|Lr|]//=.
+  - case: ifP=>///eqP-EV; rewrite (nopen_var' EQ)/=EV =>{}EQ.
+    exists d; rewrite eq_refl; split=>//.
+    rewrite addnS; by apply/leq_addr.
+  - move: (Ih _ _ EQ)=>[m][BND] LE _.
+    by exists m; split=>//; rewrite addnS.
+Qed.
+
+(* l_open d L (n_rec m L') = n_rec m (l_open (d - m) L L') ? *)
+Lemma lopen_nrec d m L
+  : l_open d L (n_rec m (l_var m)) =
+    n_rec m (if d == 0 then l_shift (d + m) 0 L else l_var m).
+Proof.
+  rewrite -{2 5} (add0n m) -{1 3}(add0n d); move: {-3 5}0=>n.
+  elim: m=>[|m Ih]/= in n *.
+  - case: (ifP (d == 0))=>[/eqP->|]; first by rewrite eq_refl !addn0.
+    by case: ifP=>//; rewrite eqn_add2l eq_sym=>->.
+  - by rewrite !addnS -!addSn Ih.
+Qed.
+
+Lemma nrec_lrecdepthI L : L = n_rec (lrec_depth L) (get_nr L).
+Proof. by elim: L=>//= L<-. Qed.
+
+Lemma nrec_twice n m L : n_rec n (n_rec m L) = n_rec (n + m) L.
+Proof. by elim n=>//= {}n->. Qed.
+
+Lemma lopen_bound d n m L :
+  m < d + n ->
+  l_open d L (n_rec n (l_var m)) = n_rec n (l_var m).
+Proof.
+  elim: n=>[|n Ih]//= in d *; last by rewrite addnS -addSn=>/Ih->.
+  by rewrite addn0 ltn_neqAle=>/andP-[/negPf->].
+Qed.
+
+Lemma lshift_nrec d r m n :
+  n < r + m ->
+  l_shift d r (n_rec m (l_var n)) = n_rec m (l_var n).
+Proof.
+  elim: m=> [|m Ih]//= in r *; first by rewrite addn0 ltnNge=>/negPf->.
+  by rewrite addnS -addSn/==>/Ih->.
+Qed.
