theories/Local/Tree.v
@@ -1,0 +1,135 @@
+From mathcomp.ssreflect Require Import all_ssreflect seq.
+From mathcomp Require Import finmap.
+
+From Paco Require Import paco paco2.
+Set Implicit Arguments.
+Unset Strict Implicit.
+Import Prenex Implicits.
+
+Require Import MPST.Common.
+
+CoInductive rl_ty :=
+| rl_end
+| rl_msg (a : l_act) (R : role) (C : lbl -> option (mty * rl_ty))
+.
+
+Definition rlty_rel := rl_ty -> rl_ty -> Prop.
+Inductive EqL_ (r : rlty_rel) : rlty_rel :=
+| el_end : @EqL_ r rl_end rl_end
+| el_msg a p C1 C2 :
+    same_dom C1 C2 ->
+    R_all r C1 C2 ->
+    @EqL_ r (rl_msg a p C1) (rl_msg a p C2).
+Hint Constructors EqL_.
+Definition EqL L1 L2 := paco2 EqL_ bot2 L1 L2.
+Derive Inversion EqL__inv with (forall r L0 L1, EqL_ r L0 L1) Sort Prop.
+
+Lemma EqL_monotone : monotone2 EqL_.
+Proof.
+  move=>L1 L2 r r' E H; elim: E =>[|a p C1 C2 D E]//; constructor=>//.
+  by move: E; rewrite /R_all=>E L Ty G G' /E-{E}E /E/H.
+Qed.
+Hint Resolve EqL_monotone.
+
+Lemma EqL_refl CL : EqL CL CL.
+Proof.
+  move: CL {-1 3}CL (erefl CL).
+  apply/paco2_acc=> r0 _ CIH CL CL'<- {CL'}.
+  apply/paco2_fold.
+  case: CL=>//a R C; constructor.
+  - by move=> Lb Ty; split=>[[CL ->]|[CL ->]]; exists CL.
+  - by move=> Lb Ty CG CG'-> [->]; right; apply: CIH.
+Qed.
+
+Lemma EqL_sym CL1 CL2 : EqL CL1 CL2 -> EqL CL2 CL1.
+Proof.
+  move: CL2 CL1; apply/paco2_acc=>r0 _ CIh L0 L1.
+  move=>/(paco2_unfold EqL_monotone); elim/EqL__inv=>// _.
+  + by move=> _ _; apply/paco2_fold; constructor.
+  + move=> a p C1 C2 DOM ALL _ _ {L0 L1}.
+    apply/paco2_fold; constructor; first by rewrite same_dom_sym.
+    move=> l Ty L L' C2l C1l; right; apply/CIh.
+    by move: (ALL l Ty _ _ C1l C2l)=>[].
+Qed.
+
+Lemma EqL_r_end_inv_aux lT lT':
+  EqL lT lT' -> lT' = rl_end -> lT = rl_end.
+Proof.
+by move=> hp; punfold hp; move: hp => [] //=.
+Qed.
+
+Lemma EqL_r_end_inv lT:
+  EqL lT rl_end -> lT = rl_end.
+Proof.
+by move=> hp; apply (EqL_r_end_inv_aux hp).
+Qed.
+
+Lemma EqL_r_msg_inv_aux lT lT' a p C':
+  EqL lT lT' -> lT' = rl_msg a p C' ->
+  exists C, same_dom C C' /\
+     R_all EqL C C' /\ lT = rl_msg a p C.
+Proof.
+move=> hp; punfold hp; move: hp => [] //=.
+move=> a0 p0 C1 C2 samed rall [eq1 eq2 eq3].
+exists C1; rewrite eq1 eq2 -eq3; split; [|split] => //=.
+rewrite /R_all; move=> L Ty lT1 lT2 ceq1 ceq2.
+rewrite /R_all in rall; move: (rall L Ty lT1 lT2 ceq1 ceq2).
+by rewrite /upaco2; elim; rewrite //=.
+Qed.
+
+Lemma EqL_r_msg_inv a p C' lT:
+  EqL lT (rl_msg a p C') ->
+  exists C, same_dom C C' /\
+     R_all EqL C C' /\ lT = rl_msg a p C.
+Proof.
+by move=> hp; apply: (EqL_r_msg_inv_aux hp).
+Qed.
+
+
+Lemma EqL_l_msg_inv_aux lT lT' a p C:
+  EqL lT lT' -> lT = rl_msg a p C ->
+  exists C', same_dom C C' /\
+     R_all EqL C C' /\ lT' = rl_msg a p C'.
+Proof.
+move=> hp; punfold hp; move: hp => [] //=.
+move=> a0 p0 C1 C2 samed rall [eq1 eq2 eq3].
+exists C2; rewrite eq1 eq2 -eq3; split; [|split] => //=.
+rewrite /R_all; move=> L Ty lT1 lT2 ceq1 ceq2.
+rewrite /R_all in rall; move: (rall L Ty lT1 lT2 ceq1 ceq2).
+by rewrite /upaco2; elim; rewrite //=.
+Qed.
+
+Lemma EqL_l_msg_inv a p C lT':
+  EqL (rl_msg a p C) lT' ->
+  exists C', same_dom C C' /\
+     R_all EqL C C' /\ lT' = rl_msg a p C'.
+Proof.
+by move=> hp; apply: (EqL_l_msg_inv_aux hp).
+Qed.
+
+Lemma EqL_trans lT1 lT2 lT3:
+  EqL lT1 lT2 -> EqL lT2 lT3 -> EqL lT1 lT3.
+Proof.
+move=> hp1 hp2; move: (conj hp1 hp2) => {hp1 hp2}.
+move=> /(ex_intro (fun lT=> _) lT2) {lT2}; move: lT1 lT3.
+apply /paco2_acc; move=> r0 _ CIH lT1 lT3; elim=> lT2.
+elim; case: lT3 =>//=.
++ move=> eql12 eql23; move: (EqL_r_end_inv eql23) eql12 =>->.
+  move=> eql12; move: (EqL_r_end_inv eql12) =>->.
+  by apply /paco2_fold; apply el_end.
++ move=> a r C eql12 eql23; move: (EqL_r_msg_inv eql23).
+  elim=> C2; elim=> samed23; elim=> rall23 lT2eq.
+  rewrite lT2eq in eql12; move: (EqL_r_msg_inv eql12).
+  elim=> C1; elim=> samed12; elim=> rall12 lT1eq.
+  rewrite lT1eq; apply /paco2_fold; apply el_msg.
+  - rewrite /same_dom; rewrite /same_dom in samed12 samed23.
+    by move=> L Ty; rewrite (samed12 L Ty).
+  - rewrite /R_all; move=> L Ty cT1 cT3 C1L C3L.
+    rewrite /upaco2; right; apply CIH.
+    have cT2aux: exists cT2, C2 L = Some (Ty, cT2).
+      rewrite /same_dom in samed12; rewrite -(samed12 L Ty).
+      by exists cT1.
+    move: cT2aux; elim=> cT2 C2L; exists cT2.
+    rewrite /R_all in rall12 rall23.
+    by split; [apply (rall12 L Ty)|apply (rall23 L Ty)].
+Qed.
