theories/Local/Unravel.v
@@ -1,0 +1,268 @@
+From mathcomp.ssreflect Require Import all_ssreflect seq.
+From mathcomp Require Import finmap.
+
+From Paco Require Import paco paco2.
+Set Implicit Arguments.
+Unset Strict Implicit.
+Import Prenex Implicits.
+
+Require Import MPST.Common.
+
+Require Import MPST.Local.Syntax.
+Require Import MPST.Local.Tree.
+
+Definition lty_rel := rel2 l_ty (fun=>rl_ty).
+Inductive l_unroll (r : lty_rel) : l_ty -> rl_ty -> Prop :=
+| lu_end :
+    @l_unroll r l_end rl_end
+| lu_rec G G' :
+    r (l_open 0 (l_rec G) G) G' ->
+    @l_unroll r (l_rec G) G'
+| lu_msg a p Ks C :
+    same_dom (find_cont Ks) C ->
+    R_all r (find_cont Ks) C ->
+    @l_unroll r (l_msg a p Ks) (rl_msg a p C)
+.
+Hint Constructors l_unroll.
+
+Scheme lunroll_ind := Induction for l_unroll Sort Prop.
+
+Lemma l_unroll_monotone : monotone2 l_unroll.
+Proof.
+  move=>IL CL r r' U H; move: IL CL U.
+  elim=>[|V|L IH|a F Ks IH] CL//=;
+    case E:_ _/ =>[|G G' R|a' F' Ks' C D U]//.
+  - by move: E R => [<-] /H; constructor.
+  - by constructor=>// l Ty IL {}CL H0 /(U _ _ _ _ H0)/H.
+Qed.
+Hint Resolve l_unroll_monotone.
+
+Definition LUnroll IL CL := paco2 l_unroll bot2 IL CL.
+
+Definition lu_unfold := paco2_unfold l_unroll_monotone.
+
+Lemma LUnroll_ind n iG cG :
+  LUnroll iG cG <-> LUnroll (lunroll n iG) cG.
+Proof.
+  split.
+  - elim: n =>[//|n Ih] in iG cG *; case: iG=>//= iL /lu_unfold.
+    by case E: _ _/ => [|L L' [|]|]//; move: E=>[->]; apply/Ih.
+  - elim: n =>// n Ih in iG cG *; case: iG=>//= G /Ih-H1.
+    by apply/paco2_fold; constructor; left.
+Qed.
+
+Lemma lunroll_end cL :
+  LUnroll l_end cL -> cL = rl_end.
+Proof. by move=> /lu_unfold-LU; case Eq: _ _ / LU. Qed.
+
+Lemma l_guarded_unroll iG :
+  l_closed (l_rec iG) -> lguarded 0 (l_rec iG) ->
+  lguarded 0 (l_open 0 (l_rec iG) iG).
+Proof.
+  move=> C GG; have GG': (lguarded 1 iG) by move:GG C=>/=; case: iG.
+  by move: (lguarded_open 0 GG C GG')=>/lguarded_depth_gt/(_ (lopen_closed C)).
+Qed.
+
+Lemma l_guarded_nunroll n iL :
+  l_closed iL -> lguarded 0 iL -> lguarded 0 (lunroll n iL).
+Proof.
+  elim: n iL=>[|n Ih]//;case=>// iG CG /(l_guarded_unroll CG)/Ih-H/=.
+  by apply/H/lopen_closed.
+Qed.
+
+Lemma l_closed_unroll n iL :
+  l_closed iL -> l_closed (lunroll n iL).
+Proof. by elim: n iL=>[|n Ih]//=; case=>//= iG /lopen_closed/Ih. Qed.
+
+Lemma v_lty G : (exists v, G = l_var v) \/ (forall v, G != l_var v).
+Proof. by case: G; try (by right); move=>v;left;exists v. Qed.
+
+Lemma lguarded_lbinds_lt s Lr :
+  l_binds s Lr = false ->
+  lguarded s Lr ->
+  lguarded s.+1 Lr.
+Proof.
+  move: {-1}(lrec_depth Lr) (erefl (lrec_depth Lr))=> n E.
+  elim: n=>[|n Ih] in s Lr E *.
+  - by case: Lr E=>//= v _ /(rwP negPf); rewrite ltn_neqAle eq_sym=>->->.
+  - case: Lr E=>//= L [/Ih-E]; apply/E.
+Qed.
+
+CoFixpoint l_expand (l : l_ty) : rl_ty :=
+  match lunroll (lrec_depth l) l with
+  | l_msg a T Ks =>
+    rl_msg a T
+           (fun l =>
+              match find_cont Ks l with
+              | Some (Ty, L) => Some (Ty, l_expand L)
+              | None => None
+              end)
+  | _ => rl_end
+  end.
+
+Lemma rltyU G : G = match G with
+                    | rl_msg a T C => rl_msg a T C
+                    | rl_end => rl_end
+                    end.
+Proof. by case: G. Qed.
+
+Fixpoint l_non_empty_cont G :=
+  match G with
+  | l_msg _ _ Ks => ~~ nilp Ks && all id [seq l_non_empty_cont K.2.2 | K <- Ks]
+  | l_rec G => l_non_empty_cont G
+  | _ => true
+  end.
+
+Definition l_precond L :=
+  l_closed L && lguarded 0 L && l_non_empty_cont L.
+
+Lemma lne_shift d n G :
+  l_non_empty_cont G ->
+  l_non_empty_cont (l_shift d n G).
+Proof.
+  elim: G=>[|v|L Ih|a p Ks Ih]//= in n *.
+  - by case: ifP.
+  - by apply/Ih.
+  - move=>/andP-[NIL NE]; apply/andP;split;first by move: Ks NIL {Ih NE}=>[].
+    rewrite -map_comp /comp/=; move: NE=>/forallbP/forall_member/member_map.
+    move=>/(_ _ ((rwP (memberP _ _)).2 _))=> H.
+    apply/forallbP/forall_member/member_map=>b /(rwP (memberP _ _))-IN.
+    by apply: (Ih _ IN _ (H _ IN)).
+Qed.
+
+Lemma lne_open n G G' :
+  l_non_empty_cont G -> l_non_empty_cont G' -> l_non_empty_cont (l_open n G' G).
+Proof.
+  move=> NE1 NE2; move: NE1.
+  elim: G n=>//.
+  - by move=> v n; rewrite /=; case: ifP=>// _ _; apply/lne_shift.
+  - by move=> G Ih n /=; apply/Ih.
+  - move=> a T C Ih n /=; case: C Ih=>//= K Ks Ih /andP-[NE_K ALL].
+    have K_in: K \in K :: Ks by rewrite in_cons !eq_refl.
+    rewrite (Ih K K_in n NE_K) /= {NE_K}.
+    move: ALL=>/forallbP/forall_member/member_map-ALL.
+    apply/forallbP/forall_member/member_map/member_map=>/=K' M.
+    move: M (ALL _ M)=>/memberP-M {}ALL.
+    have K'_in : K' \in K :: Ks by rewrite in_cons M orbT.
+    by apply/(Ih _ K'_in n)/ALL.
+Qed.
+
+Lemma lne_unr n G : l_non_empty_cont G -> l_non_empty_cont (lunroll n G).
+Proof.
+  elim: n G=>[//|n/=] Ih; case=>//= G NE.
+  have: l_non_empty_cont (l_rec G) by [].
+  by move=>/(lne_open 0 NE); apply/Ih.
+Qed.
+
+Definition l_expand' L :=
+  match L with
+  | l_msg a T Ks =>
+    rl_msg a T (fun l : lbl => match find_cont Ks l with
+                               | Some (Ty, L0) => Some (Ty, l_expand L0)
+                               | None => None
+                               end)
+  | _ => rl_end
+  end.
+
+Lemma l_expand_once L : l_expand L = l_expand' (lunroll (lrec_depth L) L).
+Proof.
+  by rewrite (rltyU (l_expand _)) /l_expand /l_expand'-rltyU-/l_expand.
+Qed.
+
+Lemma l_expand_unr L :
+  lguarded 0 L ->
+  l_closed L ->
+  l_non_empty_cont L ->
+  LUnroll L (l_expand L).
+Proof.
+  move=>gG cG NE; rewrite l_expand_once.
+  move: {-1}(l_expand' _) (erefl (l_expand' (lunroll (lrec_depth L) L))).
+  move=>CG ECG; move: L CG {ECG gG cG NE}(conj ECG (conj gG (conj cG NE))).
+  apply/paco2_acc=>r _ /(_ _ _ (conj erefl (conj _ (conj _ _))))-CIH.
+  move=> G CG [<-]{CG} [gG][cG][NE].
+  case: G cG gG NE.
+  - move=>_ _ _ /=; by apply/paco2_fold; constructor.
+  - by move=>V /lclosed_not_var/(_ V)/eqP/(_ erefl).
+  - move=>G cG gG nE /=;apply/paco2_fold.
+    constructor; right; have gG': lguarded 1 G by move: gG.
+    rewrite (lguarded_recdepth (m:=0) gG' _ (l_rec G)) //.
+    apply/CIH.
+    by apply/l_guarded_unroll.
+    by apply/lopen_closed.
+    by apply/lne_open.
+  - move=>F T C cG gG NE; apply/paco2_fold; constructor.
+    + move=>l Ty; case: find_cont=>[[Ty0 L0]|]//; split=>[][G]//[->] _.
+      * by exists (l_expand L0).
+      * by exists L0.
+    + move=> l Ty G CG FND; rewrite FND=>[][<-]; right.
+      move: cG; rewrite /l_closed/==>/flatten_eq_nil/member_map-cG.
+      move: gG; rewrite /==>/forallbP/forall_member-gG.
+      move: NE=>/==>/andP-[NE_C]/forallbP/forall_member/member_map-NE.
+      move: (find_member FND)=>MEM.
+      rewrite l_expand_once.
+      by apply/(CIH _ (gG _ MEM) (cG _ MEM) (NE _ MEM)).
+Qed.
+
+Lemma LUnroll_EqL L CL CL' : LUnroll L CL -> EqL CL CL' -> LUnroll L CL'.
+Proof.
+  move=> H1 H2; move: L CL' {H1 H2 CL} (ex_intro (fun=>_) CL (conj H1 H2)).
+  apply/paco2_acc=>r _ /(_ _ _ (ex_intro _ _ (conj _ _)))-CIH.
+  move=> L CL [CL'][LU]EQ.
+  move: LU EQ=>/(paco2_unfold l_unroll_monotone); case.
+  - move=>/(paco2_unfold EqL_monotone); case E: _ _ / =>//.
+    by apply/paco2_fold; constructor.
+  - move=> G G' [/CIH-GU|//] /GU-H.
+    by apply/paco2_fold; constructor; right.
+  - move=> a p Ks C DOM ALL; move=>/(paco2_unfold EqL_monotone).
+    case E: _ _ / =>[|a' p' CL1 CL2 DOM' EQ_ALL]//.
+    move: E DOM' EQ_ALL=>[<-<-<-] DOM' E_ALL {a' p' CL1}.
+    apply/paco2_fold; constructor; first by apply/(same_dom_trans DOM).
+    move=>l Ty G iL Cl CCl; right.
+    move: (dom DOM Cl)=>[LL]Cl'.
+    move: (ALL _ _ _ _ Cl Cl')=>[UG|//].
+    move: (E_ALL _ _ _ _ Cl' CCl)=>[EG|//].
+    by apply/(CIH _ _ _ UG EG).
+Qed.
+
+Lemma lunroll_inf Li Lr Li' :
+  lunroll (lrec_depth Li) Li = l_rec Li' ->
+  LUnroll Li Lr.
+Proof.
+  rewrite lunroll_nopen=>/nopen_rec-[m]; rewrite add0n=>[][BND].
+  rewrite {2}(nrec_lrecdepthI Li).
+  move: (getnr_nonrec Li) BND; case: (get_nr Li)=>//= v _ /eqP->.
+  move: (lrec_depth Li)=>d {v Li Li'}.
+  move EQ: (n_rec d (l_var m))=>Li LT; move: {EQ LT}(conj EQ LT)=>H.
+  move: (ex_intro (fun=>_) m (ex_intro (fun=>_) d H))=>{m d}H.
+  move: Li Lr H; apply/paco2_acc=> r _.
+  move=>/(_ _ _ (ex_intro _ _ (ex_intro _ _ (conj erefl _ ))))-CIH Li Lr.
+  move=>[m][n][<-]{Li}; case: n=>//= n LE.
+  apply/paco2_fold; constructor; move: LE; case: (boolP (n == m)).
+  - move=>/eqP-> _; rewrite lopen_nrec add0n eq_refl.
+    rewrite -/(n_rec m.+1 _) lshift_nrec // nrec_twice addnS.
+    by right; apply/CIH; apply: leq_addr.
+  - move=> H0 H1; move: {H0 H1} (conj H0 H1)=>/andP.
+    rewrite eq_sym -ltn_neqAle => LE; rewrite lopen_bound //.
+    by right; apply/CIH.
+Qed.
+
+Fixpoint expand_env (e : seq (role * l_ty)) : {fmap role -> rl_ty} :=
+  match e with
+  | [::] => [fmap]
+  | (k, v) :: t => (expand_env t).[k <- l_expand v]
+  end%fmap.
+
+Lemma in_expanded_env (e : seq (role * l_ty)) p :
+  (omap l_expand (find_cont e p) = (expand_env e).[? p])%fmap.
+Proof.
+  elim: e=>//=; first by rewrite fnd_fmap0.
+  move=>[k v] t; rewrite fnd_set /extend; case: ifP=>[/eqP->|neq].
+  + by rewrite eq_refl.
+  + by rewrite eq_sym neq.
+Qed.
+
+Lemma lunroll_isend L CL : LUnroll L CL -> l_isend L -> CL = rl_end.
+Proof.
+  move=> LU /keep_unrolling-[k END]; move: LU=>/(LUnroll_ind k).
+  by move: END=><-; apply/lunroll_end.
+Qed.
