theories/Projection/CProject.v
@@ -1,0 +1,356 @@
+From mathcomp.ssreflect Require Import all_ssreflect seq.
+From mathcomp Require Import finmap.
+
+From Paco Require Import paco paco1 paco2.
+
+Set Implicit Arguments.
+Unset Strict Implicit.
+Import Prenex Implicits.
+
+Require Import MPST.Common.
+Require Import MPST.Global.Tree.
+Require Import MPST.Local.Tree.
+
+Section CProject.
+  Definition Merge (F : lbl -> option (mty * rl_ty)) (L : rl_ty) : Prop :=
+    forall Lb Ty L', F Lb = Some (Ty, L') -> EqL L' L.
+
+  Inductive WF_ (r : rg_ty -> Prop) : rg_ty -> Prop :=
+  | WF_end : WF_ r rg_end
+  | WF_msg F T C :
+      F != T ->
+      P_all r C ->
+      (exists l Ty G, C l = Some (Ty, G)) ->
+      WF_ r (rg_msg F T C).
+  Definition WF := paco1 WF_ bot1.
+
+  Lemma WF_mon : monotone1 WF_.
+  Proof.
+    move=> G r r' [].
+    - by move=> _; apply/WF_end.
+    - by move=> F T C FT ALL NE H; apply/WF_msg=>// l Ty {}G Cl; apply/H/ALL/Cl.
+  Qed.
+
+  Definition proj_rel := rg_ty -> rl_ty -> Prop.
+  Inductive Proj_ (p : role) (r : proj_rel) : proj_rel :=
+  | prj_end G : ~ part_of p G -> WF G -> Proj_ p r G rl_end
+  | prj_send q KsG KsL :
+      p != q ->
+      same_dom KsG KsL ->
+      R_all r KsG KsL ->
+      Proj_ p r (rg_msg p q KsG) (rl_msg l_send q KsL)
+  | prj_recv q KsG KsL :
+      p != q ->
+      same_dom KsG KsL ->
+      R_all r KsG KsL ->
+      Proj_ p r (rg_msg q p KsG) (rl_msg l_recv q KsL)
+  | prj_mrg q s KsG KsL L :
+      q != s ->
+      p != q ->
+      p != s ->
+      (exists l Ty G, KsG l = Some (Ty, G)) ->
+      P_all (part_of_all p) KsG ->
+      same_dom KsG KsL ->
+      R_all r KsG KsL ->
+      Merge KsL L ->
+      Proj_ p r (rg_msg q s KsG) L
+  .
+  Hint Constructors Proj_.
+  Derive Inversion Proj__inv  with (forall p r G L, Proj_ p r G L) Sort Prop.
+
+  Lemma Proj_monotone p : monotone2 (Proj_ p).
+  Proof.
+  rewrite /monotone2; move=> x0 x1 r r' it LE; move: it; case=>//.
+  + by move=>G part; constructor.
+  + move=> q KsG KsL neq samed HP; constructor =>//; move: HP; rewrite /R_all.
+    move=> HP l Ty G L KsG_l KsL_l; apply: LE; by apply: (@HP l Ty G L KsG_l KsL_l).
+  + move=> q KsG KsL neq samed rall; constructor =>//; move: rall; rewrite /R_all.
+    move=> rall l t G L KsG_l KsL_l; apply: LE. by apply: (rall _ _ _ _ KsG_l KsL_l).
+  + move=> q s KsG KsL L0 neq_qs neq_pq neq_ps NE parts samed rall merg.
+    apply (@prj_mrg _ _ _ _ KsG KsL _) =>//; move: rall; rewrite /R_all.
+    move=> rall l t G L KsG_l KsL_l; apply: LE; by apply: (rall _ _ _ _ KsG_l KsL_l).
+  Qed.
+  Hint Resolve Proj_monotone.
+  Definition Project p CG CL := paco2 (Proj_ p) bot2 CG CL.
+
+  Lemma Project_inv (p : role) (G : rg_ty) (L : rl_ty)
+        (P : (let (sort, _) := role in sort) -> rg_ty -> rl_ty -> Prop) :
+    (forall G0, G0 = G -> rl_end = L -> ~ part_of p G0 -> WF G0 -> P p G0 rl_end) ->
+    (forall q CG CL,
+       rg_msg p q CG = G -> rl_msg l_send q CL = L ->
+       p != q -> same_dom CG CL -> R_all (Project p) CG CL ->
+       P p (rg_msg p q CG) (rl_msg l_send q CL)) ->
+    (forall q CG CL,
+       rg_msg q p CG = G -> rl_msg l_recv q CL = L ->
+       p != q -> same_dom CG CL -> R_all (Project p) CG CL ->
+       P p (rg_msg q p CG) (rl_msg l_recv q CL)) ->
+    (forall (q s : role) CG CL L0,
+        q != s -> p != q -> p != s ->
+        rg_msg q s CG = G -> L0 = L ->
+        (exists l Ty G, CG l = Some (Ty, G)) ->
+        P_all (part_of_all p) CG -> same_dom CG CL -> R_all (Project p) CG CL ->
+        Merge CL L -> P p (rg_msg q s CG) L) ->
+    Project p G L -> P p G L.
+  Proof.
+    move=> Hend Hsnd Hrcv Hmrg /(paco2_unfold (Proj_monotone (p:=p))).
+    elim/Proj__inv =>/(paco2_fold _ _ _ _); rewrite -/(Project p G L) => PRJ.
+    + by move=> G0 PART WF EQ1 EQ2; apply/Hend.
+    + move=> q CG CL pq DOM ALL EQ1 EQ2; apply/Hsnd=>//.
+      by move=>l Ty G0 G1 CGl CLl; move: (ALL l Ty G0 G1 CGl CLl)=>[|//].
+    + move=> q CG CL pq DOM ALL EQ1 EQ2; apply/Hrcv=>//.
+      by move=>l Ty G0 G1 CGl CLl; move: (ALL l Ty G0 G1 CGl CLl)=>[|//].
+    + move=> q s CG CL L0 qs pq ps NE Part DOM ALL MRG EQ1 EQ2; apply/Hmrg=>//.
+      by move=>l Ty G0 G1 CGl CLl; move: (ALL l Ty G0 G1 CGl CLl)=>[|//].
+  Qed.
+
+  Lemma samed_eql C0 C :
+    R_all EqL C0 C ->
+    same_dom C0 C ->
+    forall l Ty L,
+      C l = Some (Ty, L) -> exists L', C0 l = Some (Ty, L') /\ EqL L' L.
+  Proof.
+    move=> ALL DOM l Ty L Cl; move: (dom' DOM Cl)=>[L' C0l].
+    by move: (ALL l Ty L' L C0l Cl)=> EQ; exists L'; split.
+  Qed.
+
+  Lemma EqL_Project p G lT lT':
+    EqL lT lT' -> Project p G lT -> Project p G lT'.
+  Proof.
+  move=> eql prj; move: (conj eql prj) => {eql prj}.
+  move=> /(ex_intro (fun lT=> _) lT) {lT}.
+  move: G lT'; apply /paco2_acc; move=> r0 _ CIH G lT'.
+  move: CIH=>/(_ _ _ (ex_intro _ _ (conj _ _)))-CIH.
+  elim=> lT; elim; case lT'.
+  + move=> eql; move: (EqL_r_end_inv eql); move=>->.
+    rewrite /Project; move=> pro; move: paco2_mon; rewrite /monotone2.
+    by move=> pamo; apply (pamo _ _ _ _ _ _ _ pro).
+  + move=> a q C eql; move: (EqL_r_msg_inv eql).
+    elim=> C0; elim=> samed; elim=> rall lTeq; rewrite lTeq.
+    move=>PRJ; move: PRJ eql; elim/Project_inv=>//.
+    * move=> q0 CG CL _ [<-->->] NE1 DOM ALL EQ_L {G q0}.
+      apply/paco2_fold; constructor=>//; first by apply: (same_dom_trans DOM).
+      move=>l Ty G G' CGl Cl; move: (samed_eql rall samed Cl)=>[L' [C0l EQ_L']].
+      right; apply/CIH; first by apply/EQ_L'.
+      by apply/(ALL _ _ _ _ CGl C0l).
+    * move=> q0 CG CL _ [<-->->] NE1 DOM ALL EQ_L {G q0}.
+      apply/paco2_fold; constructor=>//; first by apply: (same_dom_trans DOM).
+      move=>l Ty G G' CGl Cl; move: (samed_eql rall samed Cl)=>[L' [C0l EQ_L']].
+      right; apply/CIH; first by apply/EQ_L'.
+      by apply/(ALL _ _ _ _ CGl C0l).
+    * move=> r s CG CL L0 NE1 NE2 NE3 _ _  NE part DOM ALL MRG.
+      move=> _ {G L0 lTeq lT}; apply/paco2_fold/prj_mrg=>//.
+      - move=>l Ty G G' CGl Cl; right; apply/CIH; first by apply/EqL_refl.
+        by apply/ALL; first by apply/CGl.
+      - move=> l Ty L' CLl; move: (MRG l Ty  L' CLl).
+        move=>/EqL_trans-H; apply: H; apply/paco2_fold; constructor=>//.
+        by move=> l0 Ty0 L0 L1 C0l0 Cl0; left; apply/(rall _ _ _ _ C0l0 Cl0).
+  Qed.
+
+  (* FIXME: abstract all g_closed && guarded ... as "wf" to simplify statements*)
+
+  Inductive IProj (p : role) : ig_ty -> rl_ty -> Prop :=
+  | iprj_end CG CL :
+      Project p CG CL ->
+      IProj p (ig_end CG) CL
+  | iprj_send1 q KsG KsL :
+      p != q ->
+      same_dom KsG KsL ->
+      R_all (IProj p) KsG KsL ->
+      IProj p (ig_msg None p q KsG) (rl_msg l_send q KsL)
+  | iprj_send2 l t q r KsG KsL L :
+      p != r ->
+      q != r ->
+      same_dom KsG KsL ->
+      R_all (IProj p) KsG KsL ->
+      KsL l = Some (t, L) ->
+      IProj p (ig_msg (Some l) q r KsG) L
+  | iprj_recv o q KsG KsL :
+      p != q ->
+      same_dom KsG KsL ->
+      R_all (IProj p) KsG KsL ->
+      IProj p (ig_msg o q p KsG) (rl_msg l_recv q KsL)
+  (* | prj_end2 G : ~ In r G -> Proj_ r G rl_end *)
+  | iprj_mrg q s KsG KsL L :
+      q != s ->
+      p != q ->
+      p != s ->
+      (* InAll r KsG -> *)
+      (exists l Ty G, KsG l = Some (Ty, G)) ->
+      same_dom KsG KsL ->
+      R_all (IProj p) KsG KsL ->
+      Merge KsL L ->
+      IProj p (ig_msg None q s KsG) L
+  .
+
+
+
+
+
+  Lemma IProj_end_inv_aux p GG CG CL:
+    IProj p GG CL -> GG = ig_end CG ->
+    Project p CG CL.
+  Proof.
+  by case=>//; move=> CG0 CL0 ipro [CGeq]; rewrite -CGeq.
+  Qed.
+
+  Lemma IProj_end_inv p CG CL:
+    IProj p (ig_end CG) CL -> Project p CG CL.
+  Proof.
+  by move=> hp; apply (IProj_end_inv_aux hp).
+  Qed.
+
+  Lemma IProj_send1_inv_aux F T C GG CL:
+    IProj F GG CL -> GG = (ig_msg None F T C) ->
+    F != T /\ (exists lC, CL = rl_msg l_send T lC /\
+    same_dom C lC /\ R_all (IProj F) C lC).
+  Proof.
+  case=>//.
+  + move=> q gC lC neq samedom rall [eq1 eq2].
+    by rewrite -eq1 -eq2; split; [| exists lC;  split; [ |]].
+  + move=> o q gC lC neq samedom rall [eq1 eq2 eq3 eq4].
+    by move: neq; rewrite eq2 -(rwP negP).
+  + move=> q s gC lC L neq1 neq2 neq3 NE samedom rall mer [eq1 eq2 eq3].
+    by move: neq2; rewrite eq1 eq_refl.
+  Qed.
+
+  Lemma IProj_send1_inv F T C CL:
+    IProj F (ig_msg None F T C) CL ->
+    F != T /\ (exists lC, CL = rl_msg l_send T lC /\
+    same_dom C lC /\ R_all (IProj F) C lC).
+  Proof.
+  by move=> hp; apply: (IProj_send1_inv_aux hp).
+  Qed.
+
+
+  Lemma IProj_send2_inv_aux L p F T C GG CL:
+    IProj p GG CL -> GG = (ig_msg (Some L) F T C) -> p != T ->
+    F != T /\ (exists lC Ty, lC L = Some (Ty, CL) /\
+    same_dom C lC /\ R_all (IProj p) C lC).
+  Proof.
+  case=>//.
+  + move=> l Ty q r gC lC CL0 neq1 neq2 samedom rall Cleq [<-<-<-<-] neq3.
+    by split=>//; exists lC, Ty; split.
+  + move=> o q gC lC neq samedom rall [_ <-<-<-] {o F T C}.
+    by rewrite eq_refl.
+  Qed.
+
+  Lemma IProj_send2_inv L p F T C CL:
+    IProj p (ig_msg (Some L) F T C) CL -> p != T ->
+    F != T /\ (exists lC Ty, lC L = Some (Ty, CL) /\
+    same_dom C lC /\ R_all (IProj p) C lC).
+  Proof.
+  by move=> hp; apply: (IProj_send2_inv_aux hp).
+  Qed.
+
+ Lemma IProj_recv_inv_aux olb F T C GG CL:
+    IProj T GG CL -> GG = (ig_msg olb F T C) ->
+    F != T /\ (exists lC, CL = rl_msg l_recv F lC /\
+    same_dom C lC /\ R_all (IProj T) C lC).
+  Proof.
+  case =>//.
+  + move=> q gC lC neq samedom rall [eq1 eq2 eq3].
+    by move: neq; rewrite eq3 -(rwP negP).
+  + move=> l Ty q r cG cL L neq1 _ _ _ _ [_ _ eq1].
+    by move: eq1 neq1=>->/eqP.
+  + move=> o q gC lC neq samedom rall [eq1 eq2 eq3].
+    by rewrite -eq2 -eq3; split; [rewrite eq_sym| exists lC; split; [ | split; [|]]].
+  + move=> q s gC lC L neq1 neq2 neq3 NE samedom rall mer [eq1 eq2 eq3 eq4].
+    by move: neq3; rewrite eq3 -(rwP negP).
+  Qed.
+
+  Lemma IProj_recv_inv olb F T C CL:
+    IProj T (ig_msg olb F T C) CL ->
+    F != T /\ (exists lC, CL = rl_msg l_recv F lC /\
+    same_dom C lC /\ R_all (IProj T) C lC).
+  Proof.
+  by move=> hp; apply: (IProj_recv_inv_aux hp).
+  Qed.
+
+  Lemma IProj_mrg_inv_aux p F T C GG CL:
+    IProj p GG CL ->
+    p != F -> p != T -> GG = ig_msg None F T C ->
+    F != T /\
+    (exists l Ty G, C l = Some (Ty, G)) /\
+    (exists lC, same_dom C lC /\
+      R_all (IProj p) C lC /\
+      Merge lC CL).
+  Proof.
+  case =>//.
+  + move=> q gC lC neq samedom rall neqF neqT [eq1 eq2 eq3].
+    by move: neqF; rewrite eq1 -(rwP negP).
+  + case=>// q cG cL neq samedom rall neqF neqT [eq1 eq2 eq3].
+    by move: neqT; rewrite eq2 -(rwP negP).
+  + move=>q s gC lC CL0 neq1 neq2 neq3 NE samedom rall mer neqF neqT [eq1 eq2 eq3].
+    split; [by move: neq1; rewrite eq1 eq2|
+            split;
+            [ by move: eq3=><-; apply/NE
+            | by exists lC; rewrite -eq3; split; [ |split; [|]]
+           ]].
+  Qed.
+
+  Lemma IProj_mrg_inv p F T C CL:
+    IProj p (ig_msg None F T C) CL ->
+    p != F -> p != T ->
+    F != T /\
+    (exists l Ty G, C l = Some (Ty, G)) /\
+    (exists lC, same_dom C lC /\
+      R_all (IProj p) C lC /\
+      Merge lC CL).
+  Proof.
+  by move=> hp neq1 neq2; apply: (IProj_mrg_inv_aux hp neq1 neq2).
+  Qed.
+
+  Lemma EqL_IProj p G lT lT':
+    IProj p G lT -> EqL lT lT' -> IProj p G lT'.
+  Proof.
+  move=> hp; move: hp lT'; elim.
+  + move=> CG {}lT Pro lT' eqL; apply: iprj_end.
+    by apply: (EqL_Project eqL Pro).
+  + move=> q C lC neq samed rall Ih lT' eqL.
+    move: (EqL_l_msg_inv eqL); elim=> lC'; elim=> samedom.
+    elim=> rall' ->; apply: (iprj_send1 neq).
+    * by move=> L Ty; rewrite (samed L Ty).
+    * move=> L Ty G0 lT0' CL lCL'.
+      move: (samedom L Ty); elim=> _.
+      elim; [move=> lT0 lCL | by exists lT0'].
+      apply: (Ih _ _ _ _ CL lCL).
+      by apply: (rall' _ _ _ _ lCL lCL').
+  + move=> L Ty q r C lC lT0 neq1 neq2 samed rall Ih lCL lT0' eqL.
+    move:(samed L Ty);elim=> _;elim;[move=> G0 CL|by exists lT0].
+    apply: (@iprj_send2 p L Ty q r C (extend L (Ty, lT0') lC) _ neq1 neq2).
+    * apply: (same_dom_extend_some_l _ samed CL).
+    * move=> LL TTy GG lTT CLL; rewrite /extend; case: ifP.
+      - rewrite -(rwP eqP); move=> eqLL [eqTy eqlT0'].
+        rewrite -eqlT0'; rewrite -eqLL in CLL.
+        move: CLL; rewrite CL; move=> [_ eqG0]; rewrite -eqG0.
+        by apply: (Ih _ _ _ _ CL lCL).
+      - by move=> neqLL lCLL; apply: rall CLL lCLL.
+    * by rewrite /extend; case: ifP =>//; rewrite eq_refl //.
+  + move=> o q C lC neq samed rall Ih lT' eqL.
+    move: (EqL_l_msg_inv eqL); elim=> lC'; elim=> samedom.
+    elim=> rall' ->; apply: (iprj_recv o neq).
+    * by move=> L Ty; rewrite (samed L Ty).
+    * move=> L Ty G0 lT0' CL lCL'.
+      move: (samedom L Ty); elim=> _.
+      elim; [move=> lT0 lCL | by exists lT0'].
+      apply: (Ih _ _ _ _ CL lCL).
+      by apply: (rall' _ _ _ _ lCL lCL').
+  + move=> q s C lC lT0 neqqs neqpq neqps NE samed rall Ih mer lT' eqL.
+    apply: (@iprj_mrg _ _ _ _
+          (same_dom_const C lT') _ neqqs neqpq neqps)=>//.
+    * by apply: same_dom_const_same_dom.
+    * move=> L Ty G0 lTT' CL sdLa.
+      move: (same_dom_const_some sdLa)=>->.
+      move: (samed L Ty); elim=> sam _; move: sam.
+      elim; [move=> lTT lCL | by exists G0].
+      by apply: (Ih _ _ _ _ CL lCL) (EqL_trans (mer _ _ _ lCL) eqL).
+    * move=> Ln Tn lTn sdc; move: (same_dom_const_some sdc) =>-> //=.
+      by apply: EqL_refl.
+  Qed.
+
+  Definition look (E : {fmap role -> rl_ty}) p := odflt rl_end E.[? p]%fmap.
+
+  Definition eProject (G: ig_ty) (E : {fmap role -> rl_ty}) : Prop :=
+    forall p, IProj p G (look E p).
+
+End CProject.
