theories/Projection/Correctness.v
@@ -1,0 +1,320 @@
+From mathcomp.ssreflect Require Import all_ssreflect seq.
+From mathcomp Require Import finmap.
+
+From Paco Require Import paco paco1 paco2.
+
+Set Implicit Arguments.
+Unset Strict Implicit.
+Import Prenex Implicits.
+
+Require Import MPST.Common.
+Require Import MPST.Global.
+Require Import MPST.Local.
+
+Require Import MPST.Projection.IProject.
+Require Import MPST.Projection.CProject.
+
+Lemma partof_all_unroll G CG p L n :
+  g_closed G ->
+  GUnroll G CG -> project simple_merge G p == Some L ->
+  depth_part n p G -> part_of_all p CG.
+Proof.
+  elim: n G CG L=>// n Ih [||G|F T C] //= CG L cG; rewrite -/prj_all.
+  - case PRJ: project=>[L0|]//; move: PRJ=>/eqP-PRJ.
+    case: ifP; first by move=>/(lbinds_depth _ PRJ)->.
+    move=> NB /gunroll_unfold; elim/gunr_inv=>// _ IG CG0 GU [EQ1] EQ2 _ DP.
+    move: EQ1 EQ2 GU DP=>//-> _ []//GU /(depthpart_open 0 (g_rec G))-DP.
+    move: NB PRJ=>/eqP-NB /eqP-PRJ; move: (project_open NB cG PRJ)=>{}/eqP-P.
+    by move: cG=>/gopen_closed/Ih/(_ GU P DP).
+  - move=>/gunroll_unfold; elim/gunr_inv=>// _ F' T' C' CC DOM UA E1 _ {CG}.
+    move: E1 DOM UA=>[->->->] DOM UA {F' T' C'}; rewrite -/(prj_all _ _).
+    case PRJ: prj_all=>[Ks|]//; case: ifP=>// FT.
+    case: ifP=>[/eqP<- _|pF]; first by constructor.
+    case: ifP=>[/eqP<- _|pT]; first by constructor.
+    move=>MRG; rewrite eq_sym pF eq_sym pT/= => DP.
+    apply: pall_cont=>l Ty CG CCl.
+    move: (dom' DOM CCl)=>[G'] Cl.
+    move: (UA _ _ _ _ Cl CCl)=>[|//].
+    move: (prj_all_find PRJ Cl)=>[L'][_]/eqP-{}PRJ GU.
+    move: (find_member Cl)=>M.
+    apply: (Ih _ _ _ _ GU PRJ).
+    * by move: cG; rewrite /g_closed/= flatten_eq_nil=>/member_map/(_ _ M).
+    * by move: DP =>/forallbP/forall_member/member_map/(_ _ M).
+Qed.
+
+Lemma partof_unroll G CG p :
+  g_closed G ->
+  guarded 0 G ->
+  GUnroll G CG ->
+  part_of p CG ->
+  p \in participants G.
+Proof.
+  move=> cG gG GU PART.
+  elim: PART=>[F T C| F T C|{}p F T C l G0 Ty Cl PART Ih] in G cG gG GU *.
+  - apply: r_in_unroll_rec_depth; move: GU=>/(GUnroll_ind (rec_depth G)).
+    move: (n_unroll (rec_depth G) G) (unroll_guarded cG gG)=>{cG gG}G NR GU.
+    move: GU NR=>/gunroll_unfold; elim/gunr_inv =>// _;
+      first by move=> IG _ _ _ _ /(_ IG); rewrite eq_refl.
+    by move=> F' T' C' CG' _ _ _ [->] _ _ _; rewrite in_cons eq_refl.
+  - apply: r_in_unroll_rec_depth; move: GU=>/(GUnroll_ind (rec_depth G)).
+    move: (n_unroll (rec_depth G) G) (unroll_guarded cG gG)=>{cG gG}G NR GU.
+    move: GU NR=>/gunroll_unfold; elim/gunr_inv =>// _;
+      first by move=> IG _ _ _ _ /(_ IG); rewrite eq_refl.
+    by move=> F' T' C' CG' _ _ _ [] _ <- _ _; rewrite in_cons orbC in_cons eq_refl.
+  - apply: r_in_unroll_rec_depth; move: GU=>/(GUnroll_ind (rec_depth G)).
+    move: (g_guarded_nunroll (rec_depth G) cG gG) (unroll_guarded cG gG).
+    move: (n_unroll (rec_depth G) G) (g_closed_unroll (rec_depth G) cG).
+    move=>{cG gG}G cG gG NR GU.
+    move: GU NR cG gG =>/gunroll_unfold; elim/gunr_inv =>// _;
+      first by move=> IG _ _ _ _ /(_ IG); rewrite eq_refl.
+    move=> F' T' C' CG' DOM UA E1 E2 _ .
+    rewrite /g_closed/==>/flatten_eq_nil/member_map-cG.
+    move=>/forallbP/forall_member=>gG.
+    move: E1 E2 cG gG DOM UA=>_ [->->->] cG gG DOM UA {G F' T' CG'}.
+    suff: p \in flatten [seq participants K.2.2 | K <- C']
+      by rewrite !in_cons=>->; rewrite orbC orbT.
+    move: (dom' DOM Cl)=>[G FND]; move: (find_member FND)=>M.
+    move: (UA _ _ _ _ FND Cl)=>[GU|//].
+    apply/flatten_mapP; exists (l, (Ty, G)); first by apply/memberP.
+    by apply/(Ih _ (cG _ M) (gG _ M) GU).
+Qed.
+
+Notation CIH4 X Y H1 H2 H3 H4 H5
+  := (ex_intro (fun=>_) X
+               (ex_intro (fun=>_) Y
+                         (conj H1 (conj H2 (conj H3 (conj H4 H5)))))).
+Lemma project_wf G p L CG :
+  g_closed G ->
+  guarded 0 G ->
+  non_empty_cont G ->
+  project simple_merge G p == Some L ->
+  GUnroll G CG -> WF CG.
+Proof.
+  move=>H1 H2 NE H3 H4; move: (CIH4 L G H1 H2 NE H3 H4)=> {H1 H2 NE H3 H4 G L}.
+  move: CG; apply/paco1_acc=>r _ /(_ _ (CIH4 _ _ _ _ _ _ _))-CIH.
+  move=> CG [L] [G] [cG [gG [NE [PRJ GU]]]]; apply/paco1_fold.
+  move: (unroll_guarded cG gG); move: PRJ=>/eqP-PRJ.
+  move: (project_unroll (rec_depth G) cG PRJ)=>[n1][n2][L'][{}PRJ] _.
+  move: GU=>/(GUnroll_ind (rec_depth G)); move: PRJ.
+  move: gG=>/(g_guarded_nunroll (rec_depth G) cG).
+  move: cG=>/(g_closed_unroll (rec_depth G)).
+  move: NE=>/(ne_unr (rec_depth G)).
+  move: (n_unroll (rec_depth G) G) => {}G; move: L'=>{}L {n1 n2}.
+  case: G =>/=; rewrite -/prj_all.
+  - by move=>_ _ _ _  /gunroll_unfold; elim/gunr_inv=>//; constructor.
+  - by move=>v /=; rewrite /g_closed/=.
+  - by move=>G _ _ _ _ _ /(_ G); rewrite eq_refl.
+  - rewrite /g_closed; move=> F T C NE /= /flatten_eq_nil/member_map-cC.
+    move=>/forallbP/forall_member-gG; rewrite -/(prj_all _ _).
+    case PRJ: prj_all =>[L'|//]; move: PRJ=>/eqP-PRJ.
+    case: ifP=>// FT _; move=>/gunroll_unfold.
+    have CNE: C != [::] by case: C NE {cC gG PRJ}.
+    have {}NE: all id [seq non_empty_cont K.2.2 | K <- C]
+      by case: C NE {CNE cC gG PRJ}.
+    move: NE=>/forallbP/forall_member/member_map-NE.
+    elim/gunr_inv => // _ F' T' C' CC DOM UA E1 _ _ {CG}.
+    move: E1 DOM UA=>[->->->] DOM UA {F' T' C'}; constructor; rewrite ?FT//.
+    * move=> l Ty G CCl; right; move: (dom' DOM CCl)=>[G']FND.
+      move: PRJ=>/eqP-PRJ; move: (prj_all_find PRJ FND)=>[L0][_]/eqP-{}PRJ.
+      move: (UA _ _ _ _ FND CCl) (find_member FND)=>[GU|//] M.
+        by apply (CIH _ _ _ (cC _ M) (gG _ M) (NE _ M) PRJ GU).
+    * case: C CNE DOM {cC gG PRJ NE UA}=>//[][l [Ty G]] Ks _.
+      have FND: find_cont ((l, (Ty, G)) :: Ks) l = Some (Ty, G)
+        by rewrite/find_cont/extend eq_refl.
+        by move=>DOM; move: (dom DOM FND)=> CCl; exists l, Ty.
+Qed.
+
+Lemma lunroll_merge r L CL CONT Ks
+      (LU : LUnroll L CL)
+      (PRJ : prj_all simple_merge CONT r = Some Ks)
+      (MRG : simple_merge L [seq K.2.2 | K <- Ks] = Some L)
+  : exists CCL,
+      same_dom (find_cont Ks) CCL /\ Merge CCL CL.
+Proof.
+  set CCL := fun l =>
+               match find_cont Ks l with
+               | Some (Ty, _) => Some (Ty, CL)
+               | None => None
+               end.
+  exists CCL; split.
+  - move=> l Ty; split=>[][G]; rewrite /CCL/=.
+    + by move=>->; exists CL.
+    + by case: find_cont=>// [][Ty' G'][<-_]; exists G'.
+  - rewrite /CCL=>l Ty L'; case: find_cont=>//[][Ty' G'][_]->.
+    by apply/EqL_refl.
+Qed.
+
+Lemma project_nonrec (r0 : proj_rel ) r CL CG L G
+      (CIH : forall cG cL iG iL,
+          g_closed iG ->
+          guarded 0 iG ->
+          non_empty_cont iG ->
+          project simple_merge iG r == Some iL ->
+          GUnroll iG cG ->
+          LUnroll iL cL ->
+          r0 cG cL)
+      (cG : g_closed G)
+      (gG : guarded 0 G)
+      (NE : non_empty_cont G)
+      (nrG : forall G' : g_ty, G != g_rec G')
+      (iPrj : project simple_merge G r = Some L)
+      (GU : GUnroll G CG)
+      (LU : LUnroll L CL)
+  : paco2 (Proj_ r) r0 CG CL.
+Proof.
+  move: (closed_not_var cG).
+  case: (boolP (r \notin participants G)); [| rewrite negbK].
+  - move=> PARTS nvG; move: iPrj=>/eqP-iPrj.
+    move: (proj1 (project_parts cG iPrj) PARTS)=> endL.
+    move: (lunroll_isend LU endL)=>->; apply/paco2_fold.
+    constructor; first by move=>/(partof_unroll cG gG GU)-P'; move: P' PARTS=>->.
+    by apply/(project_wf cG gG NE iPrj).
+  - case: G cG gG NE nrG iPrj GU=>//;
+            first by move=> GT _ _ _ /(_ GT); rewrite eq_refl.
+    move=>FROM TO CONT; rewrite project_msg /g_closed/=.
+    move=>/flatten_eq_nil/member_map-cG /forallbP/forall_member-gG.
+    move=>/andP-[NE_C /forallbP/forall_member/member_map-NE] _ I_prj GU PARTS _.
+    move: GU; move=>/gunroll_unfold.
+    case E: _ _/ =>// [FROM' TO' CONT' CC DOM GU].
+    move: E DOM GU=> [<-<-<-] {FROM' TO' CONT'} DOM GU.
+    apply/paco2_fold; move: I_prj.
+    case E: prj_all=>[KsL|]//; case:ifP=>// F_neq_T.
+    case:ifP=>[F_r | F_ne_r].
+    + move=>[EL]; move: EL LU=><- {L} /lu_unfold-LU.
+      case EL: _ _/LU=>[||a p Ks C LD LU]//; move: EL LD LU=>[<-<-<-] LD LU {a p Ks}.
+      move: (prjall_dom E)=>iDOM.
+      move: F_r CIH E=>/eqP<- CIH E; apply/prj_send; first by apply/negPf.
+      * by apply/(same_dom_trans
+                    (same_dom_trans ((same_dom_sym _ _).1 DOM) iDOM)).
+      * move=> l Ty G G' CCl Cl; right; move: (dom' DOM CCl)=>[iG FND].
+        move: (GU _ _ _ _ FND CCl)=>[{}GU|//].
+        move: (dom iDOM FND)=>[iL FND'].
+        move: (LU _ _ _ _ FND' Cl)=>[{}LU|//].
+        move: (prjall_fnd E FND FND')=>/eqP-PRJ.
+        move: (find_member FND)=>M.
+        by apply: (CIH _ _ _ _ (cG _ M) (gG _ M) (NE _ M) PRJ GU LU).
+    + case:ifP=>[T_r | T_ne_r].
+      * move=>[EL]; move: EL LU=><- {L} /lu_unfold-LU {F_ne_r}.
+        case EL: _ _/LU=>[||a p Ks C DU LU]//; move: EL DU LU=>[<-<-<-] DU LU {a p Ks}.
+        move: T_r CIH E=>/eqP<- CIH E.
+        move: (prjall_dom E)=>iDOM.
+        apply/prj_recv; first by rewrite eq_sym (F_neq_T).
+        - by apply/(same_dom_trans
+                      (same_dom_trans ((same_dom_sym _ _).1 DOM) iDOM)).
+        - move=> l Ty G G' CCl Cl; right; move: (dom' DOM CCl)=>[iG FND].
+          move: (GU _ _ _ _ FND CCl)=>[{}GU|//].
+          move: (dom iDOM FND)=>[iL FND'].
+          move: (LU _ _ _ _ FND' Cl)=>[{}LU|//].
+          move: (prjall_fnd E FND FND')=>/eqP-PRJ.
+          move: (find_member FND)=>M.
+          by apply: (CIH _ _ _ _ (cG _ M) (gG _ M) (NE _ M) PRJ GU LU).
+      * move=> MRG.
+        have M: simple_merge L [seq K.2.2 | K <- KsL] = Some L
+          by move: MRG=>{E}; case: KsL=>//=K Ks /eqP-M;
+             move: (simple_merge_some M)=>E; move: E M=>->; rewrite eq_refl=>/eqP.
+        move: (lunroll_merge LU E M)=>[CCL [DL cMRG]].
+        move: F_ne_r T_ne_r; rewrite eq_sym=>F_ne_r; rewrite eq_sym=>T_ne_r.
+        apply: prj_mrg;rewrite ?F_ne_r ?T_ne_r ?F_neq_T//; last by apply:cMRG.
+        - case: CONT NE_C DOM {cG gG NE PARTS GU E}=>// K Ks _ DOM.
+          case: K DOM=>[l [Ty G] DOM]/=.
+          have: (find_cont ((l, (Ty, G)) :: Ks) l = Some (Ty, G))
+            by rewrite /find_cont/extend !eq_refl.
+          by move=>/(dom DOM)=>[G']; exists l, Ty.
+        - move: E MRG=>/eqP-E /eqP-MRG; move: (prjall_merge E MRG)=> ALL_EQ.
+          move=> l Ty G CCl; move: (dom' DOM CCl)=>[iG iFND].
+          move: (find_member iFND)=>MEM; move: (GU _ _ _ _ iFND CCl)=>[GU'|//].
+          move: (ALL_EQ _ MEM) (cG _ MEM)=>PK cK.
+          move: PARTS; rewrite !in_cons F_ne_r T_ne_r /= => PARTS.
+          move: PARTS=> /flatten_mapP-[K] /memberP-K_CONT r_in_K.
+          move: ((project_parts_in (cG _ K_CONT) (ALL_EQ _ K_CONT)).2 r_in_K).
+          rewrite (project_depth cK PK)=>[][m] H.
+          by apply/(partof_all_unroll cK GU' PK)/H.
+        - move:DOM=>/same_dom_sym-DOM; apply/(same_dom_trans DOM).
+          by apply/(same_dom_trans _ DL)/(prjall_dom E).
+        - move=> l Ty G cL CCl CCLl; right.
+          move: (dom' DOM CCl)=>[iG iFND]; move: (find_member iFND)=>MEM.
+          move: (cG _ MEM) (gG _ MEM) (NE _ MEM)=>/= {}cG {}gG {}NE.
+          move: E MRG=>/eqP-E /eqP-MRG; move: (prjall_merge E MRG).
+          move=>/(_ _ MEM)=>/=PRJ.
+          move: (GU _ _ _ _ iFND CCl)=>[{}GU|//].
+          apply: (CIH _ _ _ _ cG gG NE PRJ GU).
+          apply/(LUnroll_EqL LU).
+          by move: (cMRG _ _ _ CCLl)=>/EqL_sym.
+Qed.
+
+Theorem ic_proj r :
+  forall iG iL cG cL,
+    g_closed iG ->
+    guarded 0 iG ->
+    non_empty_cont iG ->
+    project simple_merge iG r == Some iL ->
+    GUnroll iG cG ->
+    LUnroll iL cL ->
+    Project r cG cL.
+Proof.
+  move=> iG iL cG cL CG GG NE Prj GU LU.
+  move: (conj CG (conj GG (conj NE (conj Prj (conj GU LU)))))
+  => {CG GG Prj GU LU NE}.
+  move => /(ex_intro (fun iL=> _) iL) {iL}.
+  move => /(ex_intro (fun iG=> _) iG) {iG}.
+  move: cG cL; apply/paco2_acc=> r0 _ CIH.
+
+  move: CIH =>/(_ _ _
+                  (ex_intro _ _
+                     (ex_intro _ _
+                        (conj _ (conj _ (conj _ (conj _ (conj _ _))))))))-CIH.
+  move=> cG cL [iG] [cG'] [ciG] [giG] [NE] [iGiL] [GU LU].
+
+  move: iGiL  => /eqP-iGiL.
+  move: (project_unroll (rec_depth iG) ciG iGiL) => [U1] [U2] [L] [proj] U12.
+  move: LU =>/(LUnroll_ind U1); move: U12=>->; rewrite -LUnroll_ind=>UL.
+  move : GU (unroll_guarded ciG giG)=>/(GUnroll_ind (rec_depth iG))=>GU nrG.
+  move: (g_guarded_nunroll (rec_depth iG) ciG giG)=>guiG.
+  move: (g_closed_unroll (rec_depth iG) ciG)=>cuiG {ciG giG iGiL}.
+  move: (ne_unr (rec_depth iG) NE)=>{}NE.
+  by apply/(project_nonrec CIH cuiG guiG NE nrG proj).
+Qed.
+
+Theorem coind_proj r G L :
+  g_precond G ->
+  project simple_merge G r == Some L ->
+  Project r (g_expand G) (l_expand L).
+Proof.
+  rewrite/g_precond=>/andP-[/andP-[cG gG] NE] P.
+  move: (proj_lclosed cG P) (project_guarded P) (proj_lne NE P)=>cL gL NEl.
+  move: (g_expand_unr gG cG NE) (l_expand_unr gL cL NEl)=>{cL gL NEl}.
+  by apply/ic_proj.
+Qed.
+
+Theorem expand_eProject (g : g_ty) (e : seq (role * l_ty))
+  : eproject simple_merge g = Some e ->
+    eProject (ig_end (g_expand g)) (expand_env e).
+Proof.
+  move=>EPRJ p; constructor.
+  have PRE: g_precond g by move: EPRJ;rewrite/eproject;case:ifP.
+  move: (precond_parts PRE); case: (boolP (nilp (participants g))).
+  + move=> NOPARTS [//|END]; move: EPRJ; rewrite /eproject PRE.
+    move: (participants g) NOPARTS=>[]//= _ [<-].
+    rewrite /look -in_expanded_env/= (expand_g_end END).
+    apply/paco2_fold/prj_end; first by case E: _ / =>//.
+      by apply/paco1_fold; constructor.
+  + move=>NE _.
+    have cG: g_closed g by move: PRE=>/andP-[/andP-[cG gG] CNE].
+    have gG: guarded 0 g by move: PRE=>/andP-[/andP-[_ gG] CNE].
+    have CNE: non_empty_cont g by move: PRE=>/andP-[_ CNE].
+    have GU: GUnroll g (g_expand g) by apply/(g_expand_unr gG cG CNE).
+    move: (eproject_some EPRJ NE)=>[q [L] /eqP-PRJ'].
+    have gWF: WF (g_expand g) by apply/(project_wf cG gG CNE PRJ' GU).
+    move=>{PRJ' L q}.
+    case: (boolP (p \in participants g)).
+  - move=>PS; move: EPRJ=>/eqP/eproject_part/(_ _ PS)-PRJ.
+    rewrite /look -in_expanded_env.
+    have ->: (odflt rl_end (omap l_expand (find_cont e p)))
+    = l_expand (odflt l_end (find_cont e p))
+      by case: find_cont=>//=;rewrite (rltyU (l_expand _)).
+      by apply/coind_proj=>//; apply/eqP.
+  - move=>PARTS; have NP: ~ part_of p (g_expand g)
+            by move=> P_of; move: PARTS; rewrite (partof_unroll cG gG GU).
+    rewrite /look -in_expanded_env (fnd_not_part EPRJ PARTS)/=.
+      by apply/paco2_fold/prj_end.
+Qed.
