theories/Projection/IProject.v
@@ -1,0 +1,942 @@
+From mathcomp.ssreflect Require Import all_ssreflect seq.
+From mathcomp Require Import finmap.
+
+From Paco Require Import paco paco1 paco2.
+
+Set Implicit Arguments.
+Unset Strict Implicit.
+Import Prenex Implicits.
+
+Require Import MPST.Common.
+Require Import MPST.Global.
+Require Import MPST.Local.
+
+(*
+  LG to All:
+  comments about the new generic merge are marked
+   NMC ,
+  as in New Merge Comment
+*)
+
+Section IProject_defs.
+
+  Variables (merge : l_ty -> seq l_ty -> option l_ty).
+
+  Definition merge_all (K : seq l_ty) :=
+    match K with
+    | h :: t => merge h t
+    | _ => None
+    end.
+
+  Fixpoint project (g : g_ty) (r : role) : option l_ty :=
+    match g with
+    | g_end => Some l_end
+    | g_var v => Some (l_var v)
+    | g_rec G =>
+      match project G r with
+      | Some L => Some (if l_binds 0 L then l_end else l_rec L)
+      | None => None
+      end
+    | g_msg p q Ks =>
+      match (fix proj_all Ks r :=
+               match Ks with
+               | [::] => Some [::]
+               | K::Ks =>
+                 match project K.2.2 r, proj_all Ks r with
+                 | Some L, Some Ks => Some ((K.1, (K.2.1, L)) :: Ks)
+                 | _, _ => None
+                 end
+               end
+            ) Ks r with
+      | Some Ks => if p == q then None
+                   else if p == r then Some (l_msg l_send q Ks)
+                        else if q == r then Some (l_msg l_recv p Ks)
+                             else merge_all [seq K.2.2 | K <- Ks]
+      | None => None
+      end
+    end.
+
+  Fixpoint prj_all (Ks : seq (lbl * (mty * g_ty))) (r : role)
+    : option (seq (lbl * (mty * l_ty))) :=
+    match Ks with
+    | [::] => Some [::]
+    | K::Ks => match project K.2.2 r, prj_all Ks r with
+               | Some L, Some Ks => Some ((K.1, (K.2.1, L)) :: Ks)
+               | _, _ => None
+               end
+    end.
+
+  Lemma project_msg p q Ks r
+    : project (g_msg p q Ks) r =
+      match prj_all Ks r with
+      | Some Ks' => if p == q then None
+                   else if p == r then Some (l_msg l_send q Ks')
+                        else if q == r then Some (l_msg l_recv p Ks')
+                             else merge_all [seq K.2.2 | K <- Ks']
+      | None => None
+      end.
+  Proof. by []. Qed.
+
+  Lemma prjall_some p Ks Ks' :
+    prj_all Ks p == Some Ks' ->
+    forall K, member K Ks ->
+              exists L, member (K.1, (K.2.1, L)) Ks' /\
+                        project K.2.2 p = Some L.
+  Proof.
+    elim: Ks => [|K Ks Ih]//= in Ks' *.
+    case Kp: project => [Lp|//].
+    case Ksp: prj_all => [LKs|//]; move: Ksp=>/eqP-Ksp.
+    move=> /eqP-[Eq]; move: Eq Ih =><- Ih {Ks'} K0 [<-{K0}|].
+    - by exists Lp; split=>//=; left.
+    - by move=> /(Ih LKs Ksp K0)-[L [L_LKs PrjL]]; exists L; split=>//=; right.
+  Qed.
+
+  Lemma prjall_some2 p Ks Ks' :
+    prj_all Ks p == Some Ks' ->
+    forall K, member K Ks' ->
+              exists G, member (K.1, (K.2.1, G)) Ks /\
+                        project G p = Some K.2.2.
+  Proof.
+    elim: Ks' => [|K Ks' Ih]//= in Ks *.
+    case: Ks=>// Kg Ks/=.
+    case Kgp: project => [Lp|//].
+    case Ksp: prj_all => [Ks''|//]; move: Ksp=>/eqP-Ksp.
+    move=>/eqP-[<-{K} EqKs'']; move: EqKs'' Ksp=>->Ksp {Ks''}.
+    move=> K [<-{K}|].
+    - by exists (Kg.2.2) =>/=; split=>//; left; case: Kg {Kgp} => l [t G].
+    - move=> M; move: (Ih Ks Ksp K M)=>[G [MG prjG]].
+      by exists G; split=>//; right.
+  Qed.
+
+  Fixpoint project_all (parts : seq role) (g : g_ty)
+    : option (seq (role * l_ty))
+    := match parts with
+       | [::] => Some [::]
+       | p :: parts =>
+         match project g p, project_all parts g with
+         | Some l, Some e => Some ((p, l) :: e)
+         | _, _ => None
+         end
+       end%fmap.
+
+  Definition eproject (g : g_ty) : option (seq (role * l_ty)) :=
+    if g_precond g
+    then project_all (undup (participants g)) g
+    else None.
+
+  Lemma eproject_some g e :
+    eproject g = Some e ->
+    ~~ nilp (participants g) ->
+    exists p l, project g p = Some l.
+  Proof.
+    rewrite /eproject; case:ifP=>// _; elim: (participants g)=>//= p ps Ih.
+    case:ifP=>//.
+    - by move=> p_in_ps /Ih-{}Ih _; apply: Ih; case: ps p_in_ps.
+    - move=> _ /=.
+      by case PRJ: project=>[L|]// _ _; exists p, L.
+  Qed.
+
+  Lemma fnd_not_part g e p :
+    eproject g = Some e -> p \notin participants g -> find_cont e p = None.
+  Proof.
+    rewrite /eproject; case:ifP=>// _ PRJ; rewrite -mem_undup=>PARTS.
+    elim: (undup (participants g)) PARTS e PRJ =>//=.
+    - by move=> _ e [<-].
+    - move => q l Ih.
+      rewrite in_cons negb_or=>/andP-[pq] /Ih-{}Ih e.
+      case PRJ: project=>[L|]//.
+      case ALL: project_all=>[E|]//.
+      by move=>[<-]; rewrite /=/extend eq_sym (negPf pq); apply/Ih.
+  Qed.
+
+  Lemma eproject_part (g : g_ty) (e : seq (role * l_ty)) :
+    eproject g == Some e ->
+    forall p,
+      p \in participants g -> project g p = Some (odflt l_end (find_cont e p)).
+  Proof.
+    rewrite /eproject; case: ifP=>//WF; move: (participants g)=>p; elim:p e=>//=.
+    move=> p ps Ih E/=; case: ifP.
+    - by move=> p_in_ps /Ih-{}Ih p'; rewrite in_cons=>/orP-[/eqP->|]; apply/Ih.
+    - move=>p_not_in/=.
+      case PRJp: project=>[L|]//;case ALL: project_all=>[E'|]//.
+      move=>/eqP-[<-] q; rewrite in_cons/= /extend eq_sym.
+      by case:ifP=>[/eqP<-| _]//=; apply/Ih/eqP.
+  Qed.
+
+  Lemma prj_isend g
+    : is_end g ->
+      forall p, exists l, project g p = Some l /\ l_isend l.
+  Proof.
+    elim: g=>//.
+    - by move=> _ p; exists l_end; split.
+    - move=> G Ih /Ih-{}Ih p /=.
+      move: (Ih p)=>[L][PRJ] END; rewrite PRJ/=.
+      case: ifP=>//_; try by exists l_end.
+      by exists (l_rec L); split.
+  Qed.
+End IProject_defs.
+
+Section SimpleMerge.
+
+  Fixpoint simple_merge  (oL : l_ty) (K : seq l_ty) :=
+    match K with
+    | [::] => Some oL
+    | h::t => if h == oL then simple_merge oL t
+              else None
+    end.
+
+
+(*NMC: Next lemma is specific to the old merge*)
+  Lemma simple_merge_some (K : lbl * (mty * l_ty))
+        (Ks : seq (lbl * (mty * l_ty))) L
+    : simple_merge K.2.2 [seq K0.2.2 | K0 <- Ks] == Some L -> K.2.2 = L.
+  Proof. by elim: Ks=>[/eqP-[]//|K' Ks Ih/=]; case:ifP. Qed.
+
+(*NMC: specific to the old merge, namely the following lemmas connects
+  the old merge for local types, which is now generic, and the merge for session types,
+  which is still defined with equality of continuations*)
+
+  Lemma fun_mergeall_old f (Ks : seq (lbl * (mty * l_ty))) X
+    : injective f ->
+      merge_all simple_merge [seq f x.2.2 | x <- Ks] == Some (f X) ->
+      merge_all simple_merge [seq x.2.2 | x <- Ks] == Some X.
+  Proof.
+    case: Ks=>[//|K Ks/=] I; elim: Ks=>[|K' Ks]//=.
+    - by move=>/eqP-[/I->].
+    - by move=> Ih; case: ifP=>///eqP-[/I->]; rewrite eq_refl=>/Ih.
+  Qed.
+
+  Lemma mergeall_fun_old f (Ks : seq (lbl * (mty * l_ty))) X:
+    merge_all simple_merge [seq x.2.2 | x <- Ks] == Some X
+    -> merge_all simple_merge [seq f x.2.2 | x <- Ks] == Some (f X).
+  Proof.
+    case: Ks=>[//|K Ks/=]; elim: Ks=>[|K' Ks]//=.
+    - by move=>/eqP-[->].
+    - by move=> Ih; case: ifP=>///eqP-[->]; rewrite eq_refl=>/Ih.
+  Qed.
+
+  Lemma prjall_merge p Ks KsL L :
+    prj_all simple_merge Ks p == Some KsL ->
+    merge_all simple_merge [seq K0.2.2 | K0 <- KsL] == Some L ->
+    forall K, member K Ks -> project simple_merge K.2.2 p == Some L.
+  Proof.
+    case: KsL=>//= Kl KsL; case: Ks=>//= Kg Ks.
+    case Kg_p: project => [Lp | //]; case Ks_p: prj_all => [Ksp | //]/=.
+    move=> Eq; move: Eq Ks_p => /eqP-[<-->] /eqP-Prj Mrg {Kl Ksp}.
+    move:Mrg (simple_merge_some Mrg)=>/=Mrg Eq; move: Eq Mrg Kg_p=>->Mrg /eqP-Kg_p.
+    move=> K [<-//|]; move: Prj Mrg K {Lp Kg_p Kg}.
+    elim: Ks KsL=>//= Kg Ks Ih KsL.
+    case Kg_p: project => [Lp | //]; case Ks_p: prj_all => [Ksp | //]/=.
+    move=> Eq; move: Eq Ih Ks_p Kg_p=>/eqP-[<-]//= Ih /eqP-Prj.
+    case: ifP=>[/eqP-> {Lp}|//] /eqP-Kg_p Mrg K [<-//|].
+    by move: Prj=>/Ih/(_ Mrg K).
+  Qed.
+
+  Lemma notin_flatten (A: eqType) (p : A) Ks :
+    (forall K, member K Ks -> p \notin K) ->
+    p \notin flatten Ks.
+  Proof.
+    elim: Ks=>//=K Ks Ih H; rewrite mem_cat negb_or (H _ (or_introl erefl)) Ih//.
+    by move=> K0 M; apply/H; right.
+  Qed.
+
+  Lemma flatten_notin (A: eqType) (p : A) Ks :
+    p \notin flatten Ks ->
+    (forall K, member K Ks -> p \notin K).
+  Proof.
+    elim: Ks=>//=K Ks Ih; rewrite mem_cat negb_or=>/andP-[pK pKs] K' [<-//|].
+    by move: K'; apply/Ih.
+  Qed.
+
+  Lemma notin_parts_project Lp p G
+       (Ep : project simple_merge G p = Some Lp)
+       (NIN : p \notin participants G)
+    : p \notin partsL Lp.
+  Proof.
+  elim: G=>[|v|G Ih|q r Ks Ih] in Lp NIN Ep *; move: Ep=>[].
+  - by move<-.
+  - by move<-.
+  - move=>/=; case Ep: project=>[Lp'|//]; case: ifP=>//; first by move=>_[<-].
+      by move=> _ [<-]/=; apply/Ih.
+  - rewrite project_msg; case Ep:prj_all=>[Ks'|//]; case:ifP=>//Npq.
+    move: NIN=>/=; rewrite !in_cons !negb_or=>/andP-[N1 /andP-[N2 NIN]].
+    rewrite eq_sym (negPf N1) eq_sym (negPf N2) => M.
+    have [K MK]: (exists K, member K Ks).
+    + case: Ks Ep {Ih NIN}=>[[E]|K Ks _]//=; last (by exists K; left).
+      by move: E M=><-.
+    + move: Ep M=>/eqP-Ep /eqP-M; move: (prjall_merge Ep M)=>H.
+      move: NIN=>/flatten_notin/member_map-H' {Ep M N1 N2 Npq Ks'}.
+         by apply/(Ih _ MK); first (by apply/H'); apply/eqP/H.
+   Qed.
+
+  Lemma l_binds_notin Lp p G
+        (Ep : project simple_merge G p = Some Lp)
+        (BLp : l_binds 0 Lp)
+    : p \notin participants G.
+  Proof.
+    elim: G 0 =>[|v|G Ih|q r Ks Ih] n//= in Lp BLp Ep *.
+    - move: Ep Ih; case Prj: project=>[L|//]; move: Prj=>/eqP-Prj; case: ifP.
+      + move=> B [E]; move: E BLp=><- _.
+        by move=>/(_ _ _ B erefl).
+      + by move=>_ [E]; move: E BLp=><-/= BLp /(_ _ _ BLp erefl).
+    - move: Ep; move: (project_msg simple_merge q r Ks p)=>/=->.
+      case Prj: prj_all=>[Ks'|//]; case: ifP=>// Eqr.
+      case: ifP=>Eqp; first by move=> [E]; move: E BLp=><-.
+      case: ifP=>Erp; first by move=> [E]; move: E BLp=><-.
+      rewrite !in_cons eq_sym Eqp eq_sym Erp /==>M.
+      apply/notin_flatten/member_map=> K Mm; apply/(Ih _ Mm _ _ BLp).
+      by move: Prj M=>/eqP-Prj /eqP-M; move: (prjall_merge Prj M)=>/(_ _ Mm)/eqP.
+  Qed.
+
+  Lemma project_var_notin p G v L :
+    (L == l_end) || (L == l_var v) ->
+    project simple_merge G p == Some L ->
+    p \notin participants G.
+  Proof.
+    elim: G => [|v'|G Ih|q r Ks Ih]// in L v *.
+    - move: Ih=>/=; case Prj: project =>[Lp|//] Ih.
+      move=>/orP-[/eqP->|/eqP->]; case: ifP=>[Lp_var|]//.
+      by move: (l_binds_notin Prj Lp_var).
+    - rewrite project_msg; case E: (prj_all _ _)=>[KsL|//]; move: E=>/eqP-E/=.
+      case: ifP=>[//|/(rwP negPf)-q_ne_r].
+      case: ifP=>[/eqP->/orP-[/eqP->|/eqP->]//|/(rwP negPf)-q_ne_p].
+      case: ifP=>[/eqP->/orP-[/eqP->|/eqP->]//|/(rwP negPf)-r_ne_p].
+      do 2 rewrite in_cons negb_or; move=> L_end_var M_some.
+      do 2 rewrite eq_sym ?q_ne_p /= ?r_ne_p /=; move: M_some.
+      move: E=>/prjall_merge-E /E-Prjall.
+      apply/flatten_mapP=>[[Kg /memberP-M]].
+      by apply/negP; apply: (Ih _ M L v L_end_var); apply: Prjall.
+  Qed.
+
+  Lemma projectmsg_var n p r s Ks :
+    project simple_merge (g_msg r s Ks) p == Some (l_var n) ->
+    r != p /\ s != p /\ r != s /\
+    (forall K, member K Ks -> project simple_merge K.2.2 p == Some (l_var n)).
+  Proof.
+    rewrite project_msg; case Ksp: prj_all => [Ks'|//]; move: Ksp=>/eqP.
+    do ! case: ifP=>//; move=>s_ne_p r_ne_p r_ne_s.
+    by move=>/prjall_merge-H /H.
+  Qed.
+
+  Lemma proj_var_eq G p q v v':
+    project simple_merge G p == Some (l_var v) ->
+    project simple_merge G q == Some (l_var v') ->
+    v == v'.
+  Proof.
+    elim: G => [|n|G Ih|f t Ks Ih]// in v v' *.
+    - by move=>/eqP-[<-]/eqP-[<-].
+    - move=>/=.
+      case Pp: project =>[Lp|//]; move: Pp=>/eqP=>Pp.
+      case Pq: project =>[Lq|//]; move: Pq=>/eqP=>Pq.
+      by case: ifP.
+    - rewrite !project_msg.
+      case Pp: prj_all =>[Lp|//]; move: Pp=>/eqP=>Pp.
+      case Pq: prj_all =>[Lq|//]; move: Pq=>/eqP=>Pq.
+      case: ifP=>//f_ne_t; do ! case: ifP=>//.
+      move=> t_ne_q f_ne_q t_ne_p f_ne_p.
+      case: Ks Pp Pq Ih=>[//= /eqP-[<-] /eqP-[<-]//|K Ks/=].
+      case Pp: project =>[Lpp|//]; move: Pp=>/eqP=>Pp.
+      case Pq: project =>[Lqq|//]; move: Pq=>/eqP=>Pq.
+      case Pp': prj_all =>[Lp'|//]; move: Pp'=>/eqP=>Pp'.
+      case Pq': prj_all =>[Lq'|//]; move: Pq'=>/eqP=>Pq'.
+      move=>/eqP-[<-]/eqP-[<-].
+      move=> /(_ K (or_introl erefl))-Ih.
+      move=>/simple_merge_some-Ep /simple_merge_some-Eq; move: Ep Eq Pp Pq=>/=->->.
+      by apply: Ih.
+  Qed.
+
+  Lemma prjall_merge_cons Ks p KsL L :
+    prj_all simple_merge Ks p = Some KsL ->
+    merge_all simple_merge [seq K.2.2 | K <- KsL] = Some L ->
+    exists K, member K Ks.
+  Proof.
+    case: Ks=>//=; first by move=>[<-].
+    move=> K Ks; case Prj:project=>[L'|//]; case PrjA:prj_all=>[KL'|//].
+    by move=>_ _; exists K; left.
+  Qed.
+
+  Lemma project_binds_eq p q G Lp Lq n m :
+    project simple_merge G p = Some Lp ->
+    project simple_merge G q = Some Lq ->
+    l_binds n Lp ->
+    l_binds m Lq ->
+    l_binds n Lq.
+  Proof.
+    elim: G=>[|v|G Ih|r s Ks Ih] in Lp Lq n m *.
+    - by move=>[<-].
+    - by move=>[<-] [<-]/=.
+    - move=>/=; case Pp: project=>[Lp'|//]; case Pq: project=>[Lq'|//].
+      by case: ifP=>_ [<-]//; case: ifP=>_ [<-]//=; apply/Ih.
+    - rewrite !project_msg.
+      case PRJp: prj_all=>[KSp|//]; case PRJq: prj_all=>[KSq|//].
+      case: ifP=>// Ers; do ! (case: ifP=> _; first by move=>[<-]).
+      move=>MRGp;do ! (case: ifP=> _; first by move=>[<-]).
+      move=> MRGq; case: (prjall_merge_cons PRJp MRGp) =>[K M].
+      move: PRJq MRGq=>/eqP-Pq /eqP-Mq; move: (prjall_merge Pq Mq M)=>/eqP.
+      move: PRJp MRGp=>/eqP-Pp /eqP-Mp; move: (prjall_merge Pp Mp M)=>/eqP.
+      move: K M Lp Lq n m {Mq Mp Pp Pq Ers KSp KSq}; apply/Ih.
+  Qed.
+
+  Lemma gclosed_lclosed d G r L :
+    g_fidx d G == [::] ->
+    project simple_merge G r == Some L ->
+    l_fidx d L == [::].
+  Proof.
+    elim: G =>[|v|G Ih|p q Ks Ih] in d L *.
+    - by move=> _ /eqP-[<-].
+    - move=> /=; case: ifP=>//.
+      by move=> H _ /eqP-[<-]/=; rewrite H.
+    - move: Ih=>/=; case Eq: project =>[Lr|//]; move: Eq=>/eqP-Eq.
+      move=> /(_ d.+1 Lr)-Ih /Ih/(_ (eq_refl _))-H.
+      case: ifP=>//; first by move=> _ /eqP-[<-].
+      by move=>B /eqP-[<-]/=; apply/H.
+    - rewrite project_msg=>H1.
+      case Eq: prj_all => [Ks'|//]; case: ifP=>[//|p_neq_q]/=.
+      move: Eq=>/eqP-Eq.
+      case: ifP=>[p_eq_r /eqP-[<-]/=|p_neq_r].
+      * rewrite !flatten_eq_nil !member_map in H1 * => H1.
+        move=> K M; move: (prjall_some2 Eq M)=>[G [M' /eqP-PrjG]].
+        by apply: (Ih _ M'); first (by rewrite H1 // H2); apply: PrjG.
+      * case: ifP=>[q_eq_r /eqP-[<-]|q_neq_r /eqP].
+        + rewrite !flatten_eq_nil !member_map in H1 *=> H1 K M.
+          move: (prjall_some2 Eq M) =>[G [M' /eqP-PrjG]].
+          by apply: (Ih _ M'); first (by rewrite H1 // H2); apply: PrjG.
+        + case: Ks' Eq=>// Kl Ks' Eq /eqP/simple_merge_some<- /=.
+          case: Ks Eq Ih H1=>//= Kg Ks.
+          case Eqg: project =>[Lk|//].
+          case EqKs: prj_all =>[Ks''|//].
+          rewrite !cat_eq_nil => /eqP-[<- H2] Ih [H3 H4].
+          by apply: (Ih  Kg)=>//=; [left=>//|apply/eqP]; apply: Eqg.
+  Qed.
+
+  Lemma prjall_open r n g l Ks Ks' :
+    (forall p : lbl * (mty * g_ty),
+      member p Ks ->
+      forall s : lty_eqType,
+        project simple_merge p.2.2 r == Some s ->
+        project simple_merge (g_open n g p.2.2) r = Some (l_open n l s)) ->
+    prj_all simple_merge Ks r = Some Ks' ->
+    prj_all simple_merge [seq (K.1, (K.2.1, g_open n g K.2.2)) | K <- Ks] r
+    = Some [seq (K.1, (K.2.1, l_open n l K.2.2)) | K <- Ks'].
+  Proof.
+    elim: Ks Ks' => [|K Ks Ih]; case=>[|K' Ks']//=.
+    - by case: project; case: prj_all.
+    - move=> H. move: (H K (or_introl erefl)).
+      case: project =>// L /(_ L (eq_refl _))->.
+      move: H=>/(_ _ (or_intror _))-H; move: Ih => /(_ _ H) {H}.
+      by case: prj_all => [Ksr|//] /(_ Ksr erefl)-> [<-<-]/=.
+  Qed.
+
+  Lemma project_guarded r iG iL :
+    project simple_merge iG r == Some iL ->
+    lguarded 0 iL.
+  Proof.
+    elim: iG =>[|v|iG Ih/=|p q Ks Ih] in iL *.
+    - by move=>/= /eqP-[<-].
+    - by move=>/= /eqP-[<-].
+    - case Prj: project=>[Lr|//]; move: Prj=>/eqP/Ih-Prj.
+      case: ifP; first by move=> _ /eqP-[<-].
+      by move=> B /eqP-[<-]/=; apply/lguarded_lbinds_lt.
+    - rewrite project_msg.
+      case PrjAll: prj_all => [KsL|]//; case: ifP=>// p_n_q.
+      case: ifP=>[p_r|p_n_r]; last case: ifP=>[q_r|q_n_r].
+      + move=>/eqP-[<-]/=.
+        move: PrjAll=>/eqP/prjall_some2-PrjAll.
+        apply/forallbP/forall_member=>K M.
+        move: (PrjAll _ M)=>[g' [Mks /eqP-Prj]].
+        by apply/(Ih _ Mks _ Prj).
+      + move=>/eqP-[<-]/=.
+        move: PrjAll=>/eqP/prjall_some2-PrjAll.
+        apply/forallbP/forall_member=>K M.
+        move: (PrjAll _ M)=>[g' [Mks /eqP-Prj]].
+        by apply/(Ih _ Mks _ Prj).
+      + move=>/eqP-Mrg; move: (prjall_merge_cons PrjAll Mrg)=>[K M].
+        move: PrjAll Mrg=>/eqP-PrjAll /eqP-Mrg.
+        move: (prjall_merge PrjAll Mrg M)=> H.
+        by apply/(Ih _ M).
+  Qed.
+
+
+  Lemma project_var_parts G v r :
+    project simple_merge G r == Some (l_var v) -> r \notin participants G.
+  Proof. by apply/project_var_notin/orP/or_intror/eq_refl. Qed.
+
+
+  Lemma prj_open_binds L1 L2 G r :
+    project simple_merge G r = Some L1 ->
+    l_binds 0 L1 ->
+    project simple_merge (g_open 0 (g_rec G) G) r = Some L2 ->
+    l_isend L2.
+  Proof.
+    move=>P1 B1; have []: project simple_merge G r = Some L1 /\ l_binds 0 L1 by split.
+    move: {-2}G  {1 2}L1 =>G' L1'.
+    elim: G' 0 =>[|v|G' Ih|p q Ks' Ih] n // in L1' L2 *.
+    - by move=>[<-].
+    - by move=>[<-]/=->/=; rewrite P1 B1=> [[<-]].
+    - move=>/=; case P: project=>[L''|//].
+      case: ifP=>//; first by move=> _ [<-].
+      move=> B [<-] {L1'}/= B'.
+      case P': project=>[L1'|//].
+      case: ifP=> BL1'//; first by move=> [<-].
+      by move=>[<-]/=; move: B' P'; apply/Ih.
+    - rewrite /g_open !project_msg -/g_open.
+      case P: prj_all=>[Ks|//]; case: ifP=>//Npq.
+      do ! case: ifP=>[_ [<-]//|_].
+      move=>MRG; move: (prjall_merge_cons P MRG) =>[K M].
+      move: P MRG=>/eqP-P /eqP-MRG.
+      move: (prjall_merge P MRG M)=>/eqP-{P MRG} P B.
+      case P': prj_all=>[Ks2|//] /eqP-MRG; move: P'=>/eqP-P'.
+      move: (prjall_merge P' MRG)=>{P' MRG} /member_map/(_ _ M)/=/eqP-P'.
+      by apply/(Ih _ M n L1' L2).
+  Qed.
+
+  Lemma project_g_open_comm G1 G2 r L1 L2 k:
+    g_closed G1 ->
+    project simple_merge G1 r = Some L1 -> project simple_merge G2 r = Some L2 ->
+    project simple_merge (g_open k G1 G2) r = Some (l_open k L1 L2).
+  Proof.
+  elim: G2 G1 k L1 L2.
+  + by move=> G1 k L1 L2 gclo eq1 => //=; move=> [eq2]; rewrite -eq2 //=.
+  + move=> VAR G1 k L1 L2 gclo eq1 => //=; move=> [eq2]; rewrite -eq2 //=.
+    case: ifP=>//; move:eq1=>/eqP-eq1.
+    by move: (gclosed_lclosed gclo eq1)=>/lshift_closed-> _; apply/eqP.
+  + move=> GT IH G1 k L1 L2 gclo eq1 => //=; case Prj: project=>[LT| //=].
+    * case: ifP; move=> lbi [eq2]; rewrite //=.
+      move: (IH _ (k.+1) L1 LT gclo eq1 Prj) =>->; rewrite -eq2 //=.
+      move: (@l_binds_open 0 (k.+1) LT L1) =>-> //=.
+      + by move: lbi; case: ifP => //=.
+      + by move: eq1; rewrite (rwP eqP); apply gclosed_lclosed.
+    * move: (IH G1 (k.+1) L1 LT gclo eq1 Prj) =>->; move: eq2=><-/=.
+      move: (@l_binds_open 0 (k.+1) LT L1) =>-> //=.
+      + by move: lbi; case: ifP => //=.
+      + by move: eq1; rewrite (rwP eqP); apply gclosed_lclosed.
+  + move=> FROM TO CONT IH G1 k L1 L2 lclo eq1 eq2.
+    move: eq2; rewrite g_open_msg_rw project_msg.
+    case Pra: prj_all=>[K| //=]; case: ifP; [by rewrite //= | ].
+    move=> partdiff; case: ifP; move=> FROMr.
+    * move: FROMr partdiff; rewrite <-(rwP eqP) =>->; move=> rTO [lmsgL2].
+      rewrite project_msg; rewrite (@prjall_open r k G1 L1 CONT K).
+      - move: rTO =>->; move: eq_refl =>-> //=; rewrite <-lmsgL2.
+        by apply f_equal; (*is this really the way to do it?*)
+          rewrite l_open_msg_rw.
+      - by move=> p mem loc; rewrite <-(rwP eqP); move=> prS; apply IH; rewrite //=.
+      - by [].
+    * case: ifP; [rewrite <-(rwP eqP) | ]; move=> TOr.
+      - rewrite TOr; move=> [lmsgL2]; rewrite project_msg; rewrite (@prjall_open r k G1 L1 CONT K).
+        + move: FROMr =>->; move: eq_refl =>-> //=; rewrite <-lmsgL2.
+          by apply f_equal; rewrite l_open_msg_rw.
+        + by move=> p mem loc; rewrite <-(rwP eqP); move=> prS; apply IH; rewrite //=.
+        + by [].
+      - rewrite (rwP eqP); move=> mer; rewrite project_msg; rewrite (@prjall_open r k G1 L1 CONT K).
+        + move: partdiff =>->; move: FROMr =>->; move: TOr =>-> //=.
+          by rewrite <-map_comp; rewrite (rwP eqP); apply mergeall_fun_old.
+        + by move=> p mem loc; rewrite <-(rwP eqP); move=> prS; apply IH; rewrite //=.
+        + by [].
+  Qed.
+
+  Lemma project_open L G r
+    : l_binds 0 L == false -> g_closed (g_rec G) ->
+  project simple_merge G r = Some L -> project simple_merge (unroll G) r = Some (l_open 0 (l_rec L) L).
+  Proof.
+  move=> nlb cl prS.
+  have: project simple_merge (g_rec G) r = Some (l_rec L).
+    move: prS; rewrite //=; case Prj: project=>[LT| //=].
+    by move=> eq; move: eq Prj nlb=>[<-] Prj; case: ifP=>//=.
+  move=> prrecS; apply project_g_open_comm; rewrite //=.
+  Qed.
+
+  Lemma project_open_end_strong L G1 G r k:
+    project simple_merge G r = Some L -> project simple_merge G1 r = Some (l_end)->
+    project simple_merge (g_open k G1 G) r = Some (l_open k l_end L).
+  Proof.
+  elim: G L G1 k.
+  + by rewrite //=; move=> L G1 k [eq] pro; rewrite -eq.
+  + rewrite //=; move=> v L G1 k [eq] pro; rewrite -eq.
+    case: ifP.
+     * by rewrite -(rwP eqP) pro; move=>->//=; case: ifP; rewrite eq_refl.
+     * by rewrite //=; case: ifP.
+  + move=> G Ih L G1 k; rewrite //=; case prG: project=> [LT|] //.
+    case: ifP=> //; move=> lbi' [eq] pro'.
+    * rewrite (@Ih LT G1 (k.+1) prG pro') -eq.
+      by rewrite (@l_binds_open 0 (k.+1) LT l_end) //=; move: lbi'; case: ifP.
+    * rewrite (@Ih LT G1 (k.+1) prG pro') -eq.
+      by rewrite (@l_binds_open 0 (k.+1) LT l_end) //=; move: lbi'; case: ifP.
+  + move=> FROM TO CONT Ih L G1 k prG pro'; move: prG; rewrite g_open_msg_rw project_msg.
+    case Pra: prj_all=>[K| //=]; case: ifP; [by rewrite //= | ].
+    move=> FROMTO; case: ifP; move=> FROMr.
+    * move: FROMr FROMTO; rewrite <-(rwP eqP) =>->; move=> rTO [eq].
+      rewrite project_msg; rewrite (@prjall_open r k G1 l_end CONT K).
+      - move: rTO =>->; move: eq_refl =>-> //=; rewrite <-eq.
+        by apply f_equal; rewrite l_open_msg_rw.
+      - by move=> p mem loc; rewrite <-(rwP eqP); move=> prS; apply Ih; rewrite //=.
+      - by [].
+    * case: ifP; [rewrite <-(rwP eqP) | ]; move=> TOr.
+      - rewrite TOr; move=> [eq]; rewrite project_msg; rewrite (@prjall_open r k G1 l_end CONT K).
+        + move: FROMr =>->; move: eq_refl =>-> //=; rewrite <-eq.
+          by apply f_equal; rewrite l_open_msg_rw.
+        + by move=> p mem loc; rewrite <-(rwP eqP); move=> prS; apply Ih; rewrite //=.
+        + by [].
+      - rewrite (rwP eqP); move=> mer; rewrite project_msg; rewrite (@prjall_open r k G1 l_end CONT K).
+        + move: FROMTO =>->; move: FROMr =>->; move: TOr =>-> //=.
+          by rewrite <-map_comp; rewrite (rwP eqP); apply mergeall_fun_old.
+        + by move=> p mem loc; rewrite <-(rwP eqP); move=> prS; apply Ih; rewrite //=.
+        + by [].
+  Qed.
+
+  Lemma project_open_end L G r : l_binds 0 L -> project simple_merge G r = Some L
+    -> project simple_merge (unroll G) r = Some (l_open 0 l_end L).
+  Proof.
+  move=> lbi pro; apply project_open_end_strong; move: pro; rewrite //=.
+  by case Prj: project=>[LT| //=]; move=> eq; move: eq Prj lbi=>[<-] Prj; case: ifP.
+  Qed.
+
+  Lemma lbinds_open_end_strong L k: l_binds k L -> l_isend (l_open k l_end L).
+  Proof.
+  elim: L k=> //.
+  + by move=> v k; rewrite /l_binds -(rwP eqP)=>->/=; case: ifP; rewrite eq_refl.
+  + by move=> L ih k //=; apply ih.
+  Qed.
+
+
+  Lemma lbinds_open_end L: l_binds 0 L -> l_isend (l_open 0 l_end L).
+  Proof.
+  by apply lbinds_open_end_strong.
+  Qed.
+
+  Lemma project_unroll_isend n r G L :
+    g_closed G ->
+    project simple_merge G r = Some L ->
+    l_isend L ->
+    exists L', project simple_merge (n_unroll n G) r = Some L' /\ l_isend L'.
+  Proof.
+  elim: n=>[|n Ih]//= in G L *.
+  - by move=> closed -> H; exists L.
+  - case: G=>[|v|G|p q Ks] closed.
+    + by move=> _ _; exists l_end.
+    + by move=>[<-].
+    + move=>/=.
+      case P:project=>[L'|//]; case: ifP.
+      * move=> lbi [eq] isend. apply (@Ih _ (l_open 0 l_end L')).
+        - by rewrite /unroll; apply gopen_closed.
+        - by apply project_open_end.
+        - by apply lbinds_open_end.
+      * rewrite (rwP eqP); move=> lbi.
+        move: (project_open lbi closed P) => P1 [eq] isend.
+        apply (Ih _ (l_open 0 (l_rec L') L')); rewrite //=.
+        - by rewrite /unroll; apply gopen_closed.
+        - move: isend; rewrite -eq => //=; move=> isend; rewrite isend_open //=.
+    + by move=>-> H; exists L.
+  Qed.
+
+  Lemma project_unroll m G r L :
+    g_closed G ->
+    project simple_merge G r = Some L ->
+    (* g_closed G -> *)
+    exists n1 n2 L',
+    project simple_merge (n_unroll m G) r = Some L' /\ lunroll n1 L = lunroll n2 L'.
+    Proof.
+    move=> closed Prj; elim: m => [|m Ih]//= in G closed L Prj *; first (by exists 0,0,L).
+    move: closed Prj;case:(rec_gty G)=>[[G'->]|/(@matchGrec g_ty)->];last (by exists 0,0,L).
+    move=>/=; case Prj: project=>[L'|]//= closed.
+    case: ifP=>//.
+    + move=> lbi; move: (project_open_end lbi Prj) => Prj'.
+      move=> [U]; move: (prj_open_binds Prj lbi Prj')=>END.
+      move: closed => /gopen_closed-closed.
+      move: (project_unroll_isend m closed Prj' END)=>[L0 [-> L0_END]].
+      move: (keep_unrolling L0_END)=>[m' U_END].
+      by exists m', m', L0; split=>//; rewrite -U -U_END; case: m' {U_END}.
+    + rewrite (rwP eqP).
+      move=> nlbi [<-]{L}.
+      move: (project_open nlbi closed Prj) => Prj'.
+      move: closed => /gopen_closed-closed.
+      move: (Ih _ closed _ Prj')=>[n1] [n2] [L0] [PRJ] UNR.
+      by exists n1.+1,n2,L0.
+  Qed.
+
+  Fixpoint l_isvar L :=
+    match L with
+    | l_var v => true
+    | l_rec L => l_isvar L
+    | _ => false
+    end.
+
+  (* Depth that guarantees that we find all occurrences of p *)
+  Fixpoint depth_part n p G :=
+    match n with
+    | 0 => false
+    | m.+1 =>
+      match G with
+      | g_msg q r Ks => if (p == q) || (p == r) then true
+                        else all (depth_part m p) [seq K.2.2 | K <- Ks ]
+      | g_rec G => depth_part m p G
+      | _ => false
+      end
+    end.
+
+  Lemma depth_next n m p G :
+    n <= m ->
+    depth_part n p G ->
+    depth_part m p G.
+  Proof.
+    elim: G=>[|v|G Ih|F T C Ih]//= in n m *; case: n=>//; case m=>//.
+    - by move=>n {}m/= LE; apply/Ih.
+    - move=>n {}m/= LE; case: ifP=>//pFT /forallbP/forall_member/member_map-H.
+      apply/forallbP/forall_member/member_map=>x M.
+      by apply/(Ih _ M _ _ _ (H _ M)).
+  Qed.
+
+  Lemma lbinds_isvar n L : l_binds n L -> l_isvar L.
+  Proof. by elim: L n =>//= L Ih n /Ih. Qed.
+
+  Lemma project_depth' p G L :
+    project simple_merge G p == Some L ->
+    ~~ (l_isend L || l_isvar L) <->
+    exists n, depth_part n p G.
+  Proof.
+    elim: G =>[|v|G Ih|F T C Ih]/= in L *; try move=>/eqP[<-]/=.
+    - by split=>// [[[]//]].
+    - by split=>// [[[]//]].
+    - case PRJ: project=>[L'|]//; move: PRJ=>/eqP-PRJ.
+      case: ifP=> B /eqP-[<-]/=.
+      + split=>// [][[|n]]//= H; move: (ex_intro (fun n=>_) n H) => {n H}.
+        by move=>/(Ih _ PRJ); rewrite negb_or (lbinds_isvar B) andbC.
+      + move: (Ih _ PRJ)=>{}Ih; rewrite Ih=> {Ih B PRJ}.
+        split=>[][[|n]]//; last by exists n.
+        by exists n.+2.
+    - rewrite -/(prj_all _ _).
+      case PRJ: prj_all=>[Ks|]//; case: ifP=>// FT.
+      case: ifP=>[|].
+      + by move=>/eqP<-/eqP-[<-]; split=>// _; exists 1; rewrite /=eq_refl.
+      case: ifP=>[|].
+      + by move=>/eqP<- _/eqP-[<-];split=>//_; exists 1; rewrite /=eq_refl orbC.
+      + rewrite eq_sym=> pT; rewrite eq_sym =>pF MRG; split.
+        * move=> VAR; move: Ih=>/(_ _ _ L); rewrite VAR=>Ih.
+          move: PRJ=>/eqP-PRJ; move: (prjall_merge PRJ MRG)=>{}PRJ.
+          have {}Ih: forall K,
+              member K C -> exists n : nat, depth_part n p K.2.2
+                by move=> K M; move: PRJ Ih=>/(_ _ M)-PRJ /(_ _ M PRJ)-<-.
+          move => {PRJ VAR MRG Ks L}.
+          suff: exists n, forall K, member K C -> depth_part n p K.2.2
+                by move=>[n H]; exists n.+1=>/=; rewrite pF pT/=;
+                     apply/forallbP/forall_member/member_map.
+          move=> {FT pF pT F T}; elim: C=>[|K C IhC] in Ih *; first by (exists 0).
+          move: (Ih K (or_introl erefl))=>[n DK].
+          move: Ih=>/(_ _ (or_intror _))=>/IhC-[m] H.
+          exists (maxn n m)=> K' [<-|/H-{}DK]; apply/(depth_next _ DK).
+          by apply/leq_maxl.
+          by apply/leq_maxr.
+        * move=> [[|n]//= ]; rewrite pF pT/=.
+          move: MRG=>/eqP-MRG; move: (prjall_merge_cons PRJ MRG)=>[K M].
+          move=>/forallbP/forall_member/member_map/( _ _ M)-DP.
+          move: (ex_intro (fun n=>_) n DP); rewrite -(Ih K M L)//.
+          by move: PRJ MRG=>/eqP-PRJ /eqP-MRG; move: (prjall_merge PRJ MRG M).
+  Qed.
+
+  Lemma guarded_closed_notvar L :
+    l_closed L ->
+    lguarded 0 L ->
+    l_isvar L = false.
+  Proof.
+    rewrite /l_closed; elim: L 0=>//=.
+    - by move=> v n; case: ifP=>//; rewrite -cardfs_eq0 cardfs1.
+    - by move=>L Ih n; apply/Ih.
+  Qed.
+
+  Lemma project_depth p G L :
+    g_closed G ->
+    project simple_merge G p == Some L ->
+    ~~ l_isend L <-> exists n, depth_part n p G.
+  Proof.
+    move=> cG PRJ; split.
+    + move=>pG; move: (gclosed_lclosed cG PRJ) (project_guarded PRJ)=>cL gL.
+      move: (guarded_closed_notvar cL gL)=>/(rwP negPf)/(conj pG)/andP.
+      by rewrite -negb_or (project_depth' PRJ).
+    + by rewrite -(project_depth' PRJ) negb_or=>/andP-[].
+  Qed.
+
+  Lemma depthpart_open v n p G G' :
+    depth_part n p G ->
+    depth_part n p (g_open v G' G).
+  Proof.
+    elim: G=>[|v'|G Ih|F T C Ih]//= in n v *; case: n=>// n/=.
+    - by apply/Ih.
+    - case:ifP=>// _ /forallbP/forall_member/member_map-DP.
+      apply/forallbP/forall_member/member_map/member_map=>/= K M.
+      by apply/(Ih _ M)/DP.
+  Qed.
+
+  Lemma lbinds_depth p G L n k :
+    project simple_merge G p == Some L -> l_binds k L -> depth_part n p G = false.
+  Proof.
+    move=>/project_depth'=>[][_ /(_ (ex_intro _ n _))-H B]; move: H.
+    rewrite negb_or andbC (lbinds_isvar B)=>/=; case: depth_part=>//.
+    by move=>/(_ is_true_true).
+  Qed.
+
+  Lemma prj_all_find C p Ks l Ty G :
+    prj_all simple_merge C p = Some Ks -> find_cont C l = Some (Ty, G) ->
+    exists L, member (l, (Ty, L)) Ks /\ project simple_merge G p = Some L.
+  Proof.
+    elim: C Ks=>// [][l'][Ty']G' Ks Ih Ks' /=; rewrite /extend.
+    case PRJ: project=>[L|]//; case PRJA: prj_all=>[KsL|]//= [<-]/=.
+    case: ifP=>[/eqP->|].
+    - by move=>[-><-]; exists L; split=>//; left.
+    - by move=> ll' /(Ih _ PRJA)-[L' [M PRJ']]; exists L'; split=>//; right.
+  Qed.
+
+  Lemma project_parts' p G L :
+    project simple_merge G p == Some L ->
+    p \notin participants G ->
+    l_isend L || l_isvar L.
+  Proof.
+    elim: G L=>//=.
+    - by move=> L /eqP-[<-].
+    - by move=> v L /eqP-[<-].
+    - move=> G Ih L; case PRJ: project=>[L'|]//.
+      move: PRJ=>/eqP-PRJ EQ Part; move: (Ih _ PRJ Part)=>L'end.
+      move: EQ; case: ifP=>//=; [move=> _ /eqP-[<-]//| ].
+      by move=> _ /eqP-[<-]/=.
+    - move=> q r Ks Ih L; rewrite -/(prj_all _ _); case PRJ: prj_all=>[KsL|]//.
+      move=> EQ Part; move: Part EQ.
+      rewrite !in_cons !negb_or=>/andP-[p_ne_q /andP-[p_ne_r p_nin]].
+      move: p_nin=>/flatten_notin/member_map-NIN.
+      case: ifP=>//q_ne_r; rewrite [in q == p]eq_sym (negPf p_ne_q).
+      rewrite [in r == p]eq_sym (negPf p_ne_r) => /eqP-MRG.
+      move: (prjall_merge_cons PRJ MRG)=>[K mem].
+      apply: (Ih K mem); last by apply/NIN.
+      by move: MRG=>/eqP-MRG; move: PRJ=>/eqP/prjall_merge/( _ MRG K mem).
+  Qed.
+
+  Lemma project_parts_end p G L :
+    project simple_merge G p == Some L ->
+    l_isend L || l_isvar L ->
+    p \notin participants G.
+  Proof.
+    elim: G L=>//.
+    - move=> G Ih L /=; case PRJ: project=>[L'|//]; move: PRJ =>/eqP-PRJ.
+      case: ifP=>//.
+      + move=> /lbinds_isvar-L'var _ _; apply/(Ih L')=>//.
+        by rewrite L'var orbT.
+      + by move=> _ /eqP-[<-]/=; apply/Ih.
+    - move=>q r Ks Ih L/=; rewrite -/(prj_all _ _).
+      case PRJ: prj_all=>[KsL|//]; case: ifP=>//q_r.
+      case: ifP=>[_ /eqP-[<-]//|qp]; case: ifP=>[_ /eqP-[<-]//|rp].
+      move=>MRG H; rewrite !in_cons eq_sym qp eq_sym rp /=.
+      move: PRJ=>/eqP-PRJ; move: (prjall_merge PRJ MRG) => PRJALL.
+      move=> {MRG PRJ q_r qp rp KsL}.
+      move: Ih=>/(_ _ _ L (PRJALL _ _) H)-Ih {PRJALL H}.
+      elim: Ks Ih=>// K Ks Ih /= H.
+      rewrite mem_cat negb_or H /= ?Ih //; [|left|left] =>//.
+      by move=> p' M1 M2; apply/H; right.
+  Qed.
+
+  Lemma project_parts p G L :
+    g_closed G ->
+    project simple_merge G p == Some L ->
+    p \notin participants G <->
+    l_isend L.
+  Proof.
+    move=> cG PRJ; split.
+    + move=>pG; move: (gclosed_lclosed cG PRJ)=>cL.
+      move: (project_guarded PRJ) (project_parts' PRJ pG)=> gL.
+      by rewrite (guarded_closed_notvar cL gL) orbC.
+    + by move=>H; apply/(project_parts_end PRJ); rewrite H.
+  Qed.
+
+  Lemma project_parts_in p G L :
+    g_closed G ->
+    project simple_merge G p == Some L ->
+    ~~ l_isend L <->
+    p \in participants G.
+  Proof.
+    move=> cG pG; split.
+    - by move=> /negPf; apply/contraFT=>/(project_parts cG pG).
+    - by move=>P; apply/negPf; move:P; apply/contraTF=>/(project_parts cG pG).
+  Qed.
+
+  Lemma prjall_dom cG cL p :
+    prj_all simple_merge cG p = Some cL -> same_dom (find_cont cG) (find_cont cL).
+  Proof.
+    elim: cG cL=>//=.
+    - by move=>cL [<-]/= l Ty; split=>[][G].
+    - move=> [l P] Ks Ih cL; case: project=>[L|]//.
+      case ALL: prj_all=>[CL|]//[<-] l' Ty'/=; move: ALL=>/Ih-{}Ih.
+      split=>[][G]; rewrite /extend; case: ifP=>_.
+      + by move=> [->]/=; exists L.
+      + by move=>/(dom Ih).
+      + by move=>[<-] _; exists P.2; case: P.
+      + by move=>/(dom' Ih).
+  Qed.
+
+  Lemma prjall_fnd cG cL p G Ty L l :
+    prj_all simple_merge cG p = Some cL ->
+    find_cont cG l = Some (Ty, G) -> find_cont cL l = Some (Ty, L) ->
+    project simple_merge G p = Some L.
+  Proof.
+    elim: cG cL=>//=.
+    - move=> [l' [Ty' G']] Ks Ih cL; case PRJ: project=>[L'|]//.
+      case ALL: prj_all=>[cL'|]// [<-] {cL}.
+      rewrite /extend; case: ifP.
+      + by move=>/eqP-> [<-<-]/=; rewrite /extend eq_refl=>[][<-].
+      + by move=>NEQ FND1 /=; rewrite /extend NEQ; apply/Ih.
+  Qed.
+
+  Lemma simple_merge_equal L Ks :
+    simple_merge L [seq K.2.2 | K <- Ks] = Some L ->
+    forall (K : (lbl * (mty  * l_ty))), member K Ks -> K.2.2 = L.
+  Proof.
+    elim: Ks=>//= K Ks Ih; case: ifP=>//.
+    by move=>/eqP-Kl /Ih-{}Ih K0 [<-|/Ih].
+  Qed.
+
+  Lemma proj_lclosed G p L : g_closed G -> project simple_merge G p == Some L -> l_closed L.
+  Proof.
+    rewrite /g_closed/l_closed; move: 0.
+    elim: G => [| v | {}G Ih | F T C Ih]/= in L *; rewrite -/prj_all.
+    - by move=>n _ /eqP-[<-].
+    - by move=>n H /eqP-[<-]/=.
+    - move=>n /Ih-{}Ih; case PRJ: project=>[L'|//].
+      case: ifP;[move=>_/eqP-[<-]//|move=>_ /eqP-[<-]/=].
+      by apply/Ih/eqP.
+    - move=>n /flatten_eq_nil/member_map-cG; rewrite -/(prj_all _ _).
+      case ALL: prj_all=>[CL|//]; move: ALL=>/eqP-ALL; do ! case: ifP=>// _.
+      + move=>/eqP-[<-]/=; apply/flatten_eq_nil/member_map=> K M.
+        move: (prjall_some2 ALL M)=>[G][MG]/eqP-PRJ.
+        by apply/(Ih _ MG _ _ (cG _ MG) PRJ).
+      + move=>/eqP-[<-]/=; apply/flatten_eq_nil/member_map=> K M.
+        move: (prjall_some2 ALL M)=>[G][MG]/eqP-PRJ.
+        by apply/(Ih _ MG _ _ (cG _ MG) PRJ).
+      + move=>MRG; move: (prjall_merge ALL MRG)=>PRJ.
+        move: ALL MRG=>/eqP-ALL /eqP-MRG; move: (prjall_merge_cons ALL MRG).
+        by move=>[K]M; apply/(Ih _ M _ _ (cG _ M) (PRJ _ M)).
+  Qed.
+
+  Lemma proj_lne G p L :
+    non_empty_cont G -> project simple_merge G p == Some L -> l_non_empty_cont L.
+  Proof.
+    rewrite /g_closed/l_closed.
+    elim: G => [| v | {}G Ih | F T C Ih]/= in L *; rewrite -/prj_all.
+    - by move=>_ /eqP-[<-].
+    - by move=>H /eqP-[<-]/=.
+    - move=>/Ih-{}Ih; case PRJ: project=>[L'|//].
+      case: ifP;[move=>_/eqP-[<-]//|move=>_ /eqP-[<-]/=].
+      by apply/Ih/eqP.
+    - move=>/andP-[NE]; rewrite -/(prj_all _ _).
+      case ALL: prj_all=>[CL|//]; move: (prjall_dom ALL).
+      move=>/samedom_nilp/contra/(_ NE)=>nilCL; move: ALL=>/eqP-ALL.
+      move=>/forallbP/forall_member/member_map=>{}NE.
+      do ! case: ifP=>// _.
+      + move=>/eqP-[<-]/=; rewrite nilCL/=.
+        apply/forallbP/forall_member/member_map=> K M.
+        move: (prjall_some2 ALL M)=>[G][MG]/eqP-PRJ.
+        by apply (Ih _ MG _ (NE _ MG) PRJ).
+      + move=>/eqP-[<-]/=; rewrite nilCL/=.
+        apply/forallbP/forall_member/member_map=> K M.
+        move: (prjall_some2 ALL M)=>[G][MG]/eqP-PRJ.
+        by apply (Ih _ MG _ (NE _ MG) PRJ).
+      + move=>MRG; move: (prjall_merge ALL MRG)=>PRJ.
+        move: ALL MRG=>/eqP-ALL /eqP-MRG; move: (prjall_merge_cons ALL MRG).
+        by move=>[K]M; apply/(Ih _ M _ (NE _ M) (PRJ _ M)).
+  Qed.
+
+End SimpleMerge.
